the SoftBound proof is done.
The admitted lemmas in SoftBound/sb_db_*.v and SoftBound/sbop_seop.v are
unrelated to the current SoftBound proofs, which are proofs for a
big-step specification designed at the earlier stage, and it turned out
that big-step makes the proofs harder, so we switched to small-step
semantics (sb_ds_*.v and sbop_dsop.v). The final version is based on the
small-step operational semantics. 

Notes for simplifying proofs
1) define a generic evaluation rules for br and br_cond
2) define a generic evaluation rules for all unop, bop, and nary-op
3) the SBpass is designed in a monadic programming style, for each of
function, we can prove some declarative intro/elim/inv lemmas, which are
useful when constructing and destructing these functions. 

Plus, we may be able to strengthen the current monads to be 'dependent'
s.t. carrying some properties of imperative changing states.
4) define fast and efficient tactics to solve goals with Ex, for
example, all the simulation proofs have goals with Ex.

Stat: (unit: line)
ssa/*.ott                         1987
ssa/*.v                          18093
ssa/compcert/*.v (our extension ) 3176
TV/*.v                           14801
SoftBound/sb_ds*.v               18927
Ocaml code                        5184
Ocaml-LLVM binding             unknown

SoftBound/sb_db*.v(with admitts)  8734



git-svn-id: https://webdav.seas.upenn.edu/svn/sol/vol@3025 eef5ea85-cc2e-0410-bd84-0fae1f012da8

src/SoftBound/sb_ds_sim.v
@@ -20,6 +20,7 @@ Require Import Znumtheory.
 Require Import sb_ds_def.
 Require Import sb_ds_trans.
 Require Import sb_ds_metadata.
+Require Import sb_ds_gv_inject.
 Require Import ssa_static.
 Require Import ssa_props.
 Require Import ssa_wf.
@@ -30,19 +31,15 @@ Ltac zeauto := eauto with zarith.
 
 Import SB_ds_pass.
 
-Definition sb_fnattrs := fnattrs_intro linkage_external visibility_default 
-  callconv_ccc nil nil.
-
-
 (* Freshness *)
 
 Definition getValueID (v:value) : atoms :=
 match v with
 | value_id id => {{id}}
-| value_const (const_gid _ id) => {{id}}
 | value_const _ => {}
 end.
 
+(*
 Fixpoint getParamsOperand (lp:params) : atoms :=
 match lp with
 | nil => {}
@@ -53,9 +50,8 @@ Definition getCmdOperands (i:cmd) : atoms :=
 match i with
 | insn_bop _ _ _ v1 v2 => getValueID v1 `union` getValueID v2
 | insn_fbop _ _ _ v1 v2 => getValueID v1 `union` getValueID v2
-(* | insn_extractelement _ _ v _ => getValueID v
+| insn_extractelement _ _ v _ => getValueID v
 | insn_insertelement _ _ v1 _ v2 _ => getValueID v1 `union` getValueID v2
-*)
 | insn_extractvalue _ _ v _ => getValueID v
 | insn_insertvalue _ _ v1 _ v2 _ => getValueID v1 `union` getValueID v2
 | insn_malloc _ _ v _ => getValueID v
@@ -75,6 +71,7 @@ match i with
 end.
 
 Definition getCmdIDs (c:cmd) := {{getCmdLoc c}} `union` getCmdOperands c.
+*)
 
 Definition id_fresh_in_value v1 i2 : Prop :=
 match v1 with
@@ -99,12 +96,13 @@ match rm with
 | nil => True
 | (id0,(bid,eid))::rm' => 
     id0 <> bid /\ id0 <> eid /\ bid <> eid /\ 
-    id0 `notin` dom rm' `union` codom rm' /\
+    id0 `notin` codom rm' /\
     bid `notin` dom rm' `union` codom rm' /\
     eid `notin` dom rm' `union` codom rm' /\
     rm_codom_disjoint rm' 
 end.
 
+(*
 Definition wf_fresh ex_ids c rm : Prop :=
 AtomSetImpl.inter (getCmdIDs c) (codom rm) [<=] {} /\
 getCmdLoc c `notin` getCmdOperands c /\
@@ -116,6 +114,7 @@ match cs with
 | nil => True
 | c::cs' => wf_fresh ex_ids c rm2 /\ wf_freshs ex_ids cs' rm2 
 end.
+*)
 
 Lemma notin_codom__neq : forall rm d id0 id1 bid eid,
   AtomSetImpl.inter d (codom rm) [<=] {} ->
@@ -133,6 +132,7 @@ Proof.
         clear - J1. fsetdec.
 Qed.
 
+(*
 Lemma notin_codom__neq' : forall rm d id1 bid eid,
   AtomSetImpl.inter d (codom rm) [<=] {} ->
   Some (bid, eid) = lookupAL _ rm id1 ->
@@ -147,6 +147,7 @@ Proof.
       eapply IHrm in J2; eauto.
         clear - J1. fsetdec.
 Qed.
+*)
 
 Lemma ids2atoms_dom : forall x d,
   In x d <-> x `in` ids2atoms d.
@@ -271,7 +272,7 @@ Proof.
   apply rmap_lookupAL in H0.
   fsetdec.
 Qed.
-
+(*
 Lemma tmp_is_fresh_rm : forall id1 ex_ids tmp ex_ids' bid eid rm c,
   wf_fresh ex_ids c rm ->
   Some (bid, eid) = lookupAL _ rm id1 ->
@@ -310,6 +311,7 @@ Proof.
       apply ids2atoms_dom; auto.              
     fsetdec.
 Qed.
+*)
 
 Lemma mk_tmp_inc : forall ex_ids ex_ids3 ex_ids5 tmp,
   incl ex_ids ex_ids3 ->
@@ -322,6 +324,7 @@ Proof.
   simpl. auto.
 Qed.
 
+(*
 Lemma wf_freshs__mk_tmp : forall cs ex_ids rm2 ptmp ex_ids1,
   wf_freshs ex_ids cs rm2 ->
   (ptmp, ex_ids1) = mk_tmp ex_ids ->
@@ -331,45 +334,9 @@ Proof.
     destruct H as [J1 J2].
     split; eauto using wf_fresh__mk_tmp.
 Qed.
+*)
 
 (* Simulation *)
-
-Definition meminj_no_overlap (f: meminj) (m: mem) : Prop :=
-  forall b1 b1' delta1 b2 b2' delta2,
-  b1 <> b2 ->
-  f b1 = Some (b1', delta1) ->
-  f b2 = Some (b2', delta2) ->
-  b1' <> b2'.
-
-Lemma meminj_no_overlap__implies : forall f m,
-  meminj_no_overlap f m -> Mem.meminj_no_overlap f m.
-Proof.
-  intros f m J.
-  unfold meminj_no_overlap in J.
-  unfold Mem.meminj_no_overlap.
-  eauto.
-Qed.
-
-Record wf_sb_mi maxb mi Mem1 Mem2 := mk_wf_sb_mi {
-  Hno_overlap : meminj_no_overlap mi Mem1;
-  Hnull : mi Mem.nullptr = Some (Mem.nullptr, 0);
-  Hmap1 : forall b, b >= Mem.nextblock Mem1 -> mi b = None;
-  Hmap2 : forall b1 b2 delta2, 
-    mi b1 = Some (b2, delta2) -> b2 < Mem.nextblock Mem2;
-  mi_freeblocks: forall b, ~(Mem.valid_block Mem1 b) -> mi b = None;
-  mi_mappedblocks: forall b b' delta, 
-    mi b = Some(b', delta) -> Mem.valid_block Mem2 b';
-  mi_range_block: forall b b' delta, 
-    mi b = Some(b', delta) -> delta = 0;
-  mi_bounds: forall b b' delta, 
-    mi b = Some(b', delta) -> Mem.bounds Mem1 b = Mem.bounds Mem2 b';
-  mi_globals : forall b, b <= maxb -> mi b = Some (b, 0)
-  }.
-
-Definition gv_inject (mi: Values.meminj) (gv gv':GenericValue) : Prop :=
-let '(vals,mks) := List.split gv in 
-let '(vals',mks') := List.split gv' in 
-val_list_inject mi vals vals'.
 
 Definition reg_simulation (mi:Values.meminj) TD gl (F:fdef) 
   (rm1:SBopsem.rmetadata) (rm2:rmap) (lc1 lc2:GVMap) : Prop :=
@@ -387,21 +354,8 @@ Definition reg_simulation (mi:Values.meminj) TD gl (F:fdef)
     getOperandValue TD ev2 lc2 gl = Some egv2 /\
     gv_inject mi bgv1 bgv2 /\
     gv_inject mi egv1 egv2
-).
-
-Fixpoint wf_global (maxb:Values.block) (gv:GenericValue) 
-  : Prop :=
-match gv with
-| nil => True
-| (Vptr b _,_)::gv' => b <= maxb /\ wf_global maxb gv'
-| _::gv' => wf_global maxb gv'
-end.
-
-Fixpoint wf_globals maxb (gl:GVMap) : Prop :=
-match gl with
-| nil => True
-| (_,gv)::gl' => wf_global maxb gv /\ wf_globals maxb gl'
-end.
+) /\
+(forall i0 gv1, lookupAL _ lc1 i0 = Some gv1 -> In i0 (getFdefLocs F)).
 
 Definition mem_simulation (mi:Values.meminj) TD (mgb:Values.block) 
   (MM1:SBopsem.mmetadata) (Mem1 Mem2:mem) : Prop :=
@@ -486,7 +440,7 @@ Definition sbEC_simulates_EC_tail (TD:TargetData) Ps1 gl (mi:Values.meminj)
          reg_simulation mi TD gl f1 rm1 rm2 lc1 lc2 /\
          incl ex_ids ex_ids3 /\ 
          call_suffix i0 nr ca t0 v p rm2 = Some cs22 /\
-         wf_freshs ex_ids3 cs13 rm2 /\
+         (*wf_freshs ex_ids3 cs13 rm2 /\*)
          trans_cmds ex_ids3 rm2 cs13 = Some (ex_ids4,cs23) /\
          trans_terminator rm2 tmn1 = Some cs24 /\
          cs2 = cs22 ++ cs23 ++ cs24
@@ -516,7 +470,7 @@ Definition sbEC_simulates_EC_head (TD:TargetData) Ps1 gl (mi:Values.meminj)
          gen_metadata_fdef nts (getFdefLocs f1) nil f1 = Some (ex_ids, rm2) /\
          reg_simulation mi TD gl f1 rm1 rm2 lc1 lc2 /\
          incl ex_ids ex_ids3 /\ 
-         wf_freshs ex_ids3 cs12 rm2 /\
+         (*wf_freshs ex_ids3 cs12 rm2 /\*)
          trans_cmds ex_ids3 rm2 cs12 = Some (ex_ids4,cs22) /\
          trans_terminator rm2 tmn1 = Some cs23 /\
          cs2 = cs22 ++ cs23
@@ -596,7 +550,7 @@ match goal with
   destruct F2 as [fh2 bs2];
   destruct HsimEC as [Hclib [HBinF [HFinPS [Htfdef [Heq0 [Hasim [Hnth [Heqb1 
     [Heqb2 [ex_ids [rm2 [ex_ids3 [ex_ids4 [cs22 [cs23 [Hgenmeta [Hrsim [Hinc 
-    [Hfresh [Htcmds [Httmn Heq2]]]]]]]]]]]]]]]]]]]]]; subst
+    [Htcmds [Httmn Heq2]]]]]]]]]]]]]]]]]]]]; subst
 end.
 
 Fixpoint params_simulation TD gl mi lc2 
@@ -635,23 +589,6 @@ match (re1, re2) with
     incomingValues_simulation mi re1' rm2 re2'
 | _ => False
 end.
-
-Definition defined_gv (gv:GenericValue) : Prop :=
-match gv with
-| (v,_)::_ => v <> Vundef
-| _ => True
-end.
-
-Fixpoint defined_gvs (gvs:list GenericValue) : Prop :=
-match gvs with
-| gv::gvs' => defined_gv gv /\ defined_gvs gvs'
-| nil => True
-end.
-
-Definition chunk_matched (gv gv':GenericValue) : Prop :=
-let '(_,ms):=split gv in
-let '(_,ms'):=split gv' in
-ms = ms'.
 
 Definition nondet_state sbSt (St : LLVMopsem.State) : Prop :=
   match sbSt, St with 
@@ -755,7 +692,7 @@ match goal with
   destruct F2 as [fh2 bs2];
   destruct HsimEC as [Hclib [HBinF [HFinPs [Htfdef [Heq0 [Hasim [Hnth [Heqb1 
     [Heqb2 [ex_ids [rm2 [ex_ids3 [ex_ids4 [cs22 [cs23 [Hgenmeta [Hrsim [Hinc 
-    [Hfresh [Htcmds [Httmn Heq2]]]]]]]]]]]]]]]]]]]]]; subst
+    [Htcmds [Httmn Heq2]]]]]]]]]]]]]]]]]]]]; subst
 end.
 
 Ltac destruct_ctx_return :=
@@ -801,14 +738,14 @@ match goal with
   destruct F2 as [fh2 bs2];
   destruct HsimEC as [Hclib [HBinF [HFinPs [Htfdef [Heq0 [Hasim [Hnth [Heqb1 
     [Heqb2 [ex_ids [rm2 [ex_ids3 [ex_ids4 [cs22 [cs23 [Hgenmeta [Hrsim [Hinc 
-    [Hfresh [Htcmds [Httmn Heq2]]]]]]]]]]]]]]]]]]]]]; subst;
+    [Htcmds [Httmn Heq2]]]]]]]]]]]]]]]]]]]]; subst;
   destruct F' as [fh1' bs1'];
   destruct F2' as [fh2' bs2'];
   destruct c'; try solve [inversion HsimEC'];
   destruct HsimEC' as [Hclib' [HBinF' [HFinPs' [Htfdef' [Heq0' [Hasim' [Hnth' 
     [Heqb1' [Heqb2' [ex_ids' [rm2' [ex_ids3' [ex_ids4' [cs22' [cs23' [cs24' 
-    [Hgenmeta' [Hrsim' [Hinc' [Hcall' [Hfresh' [Htcmds' [Httmn' Heq2']]]]]]]]]]]]
-    ]]]]]]]]]]]; 
+    [Hgenmeta' [Hrsim' [Hinc' [Hcall' [Htcmds' [Httmn' Heq2']]]]]]]]]]]]
+    ]]]]]]]]]]; 
     subst
 end.
 
