src/SoftBound/sb_ds_trans_lib.v
@@ -25,6 +25,7 @@ Require Import ssa_props.
 Require Import ssa_wf.
 Import SB_ds_pass.
 Require Import sb_ds_sim.
+Require Import sb_ds_gv_inject.
 Require Import sb_ds_trans_axioms.
 
 Ltac zauto := auto with zarith.
@@ -51,72 +52,6 @@ Proof.
       auto.
 Qed.
 
-Lemma reg_simulation__updateAddAL_lc : forall mi TD gl f1 rm1 rm2 lc1 lc2 i0 gv 
-    gv',
-  reg_simulation mi TD gl f1 rm1 rm2 lc1 lc2 ->
-  In i0 (getFdefLocs f1) ->
-  i0 `notin` codom rm2 ->
-  gv_inject mi gv gv' ->
-  reg_simulation mi TD gl f1 rm1 rm2 (updateAddAL GenericValue lc1 i0 gv)
-    (updateAddAL GenericValue lc2 i0 gv').
-Proof.
-  intros mi TD gl f1 rm1 rm2 lc1 lc2 i0 gv gv' Hsim Hin Hnotin. 
-  destruct Hsim as [J1 J2].    
-  split.
-    intros i1 gv1 J.
-    destruct (id_dec i0 i1); subst.
-      rewrite lookupAL_updateAddAL_eq in *; auto.
-      inv J. exists gv'. auto.
-    
-      rewrite <- lookupAL_updateAddAL_neq in J; auto.
-      rewrite <- lookupAL_updateAddAL_neq; auto.
-
-    intros vp bgv1 egv1 J.
-    apply J2 in J. 
-    destruct J as [bv2 [ev2 [bgv2 [egv2 [J11 [J12 [J13 [J14 J15]]]]]]]].
-    exists bv2. exists ev2. exists bgv2. exists egv2.
-    split; auto.
-    destruct vp as [pid |]; simpl in J11.
-      case_eq (lookupAL (id * id) rm2 pid).
-        intros [bid eid] J.
-        rewrite J in J11.    
-        inv J11.
-        simpl.
-        assert (J':=J).
-        apply in_codom_of_rmap in J'.    
-        destruct J' as [J16 J17].      
-        rewrite <- lookupAL_updateAddAL_neq; try solve [fsetdec].
-        rewrite <- lookupAL_updateAddAL_neq; try solve [fsetdec].
-        repeat (split; auto).
-
-        intro J.
-        rewrite J in J11. inversion J11.
-
-      case_eq (get_const_metadata c).
-        intros [bc ec] J.
-        rewrite J in J11.
-        inv J11.
-        simpl in *.
-        repeat (split; auto).
-
-        intro J.  rewrite J in J11.
-        inv J11. simpl in *.
-        repeat (split; auto).
-Qed.
-
-Lemma gv_inject_incr:
-  forall f1 f2 v v',
-  inject_incr f1 f2 ->
-  gv_inject f1 v v' ->
-  gv_inject f2 v v'.
-Proof.
-  intros. 
-  unfold gv_inject in *.
-  destruct (split v).
-  destruct (split v').
-  eauto using val_list_inject_incr.
-Qed.
-
 Lemma inject_incr__preserves__reg_simulation : forall mi TD fl F rm1 rm2 lc1 lc2
     mi',
   reg_simulation mi TD fl F rm1 rm2 lc1 lc2 ->
@@ -124,1776 +59,15 @@ Lemma inject_incr__preserves__reg_simulation : forall mi TD fl F rm1 rm2 lc1 lc2
   reg_simulation mi' TD fl F rm1 rm2 lc1 lc2.
 Proof.
   intros mi TD fl F rm1 rm2 lc1 lc2 mi' Hrsim Hinc.
-  destruct Hrsim as [J1 J2].
+  destruct Hrsim as [J1 [J2 J3]].
   split.
     intros. apply J1 in H. destruct H as [gv2 [H1 H2]].
     exists gv2. split; eauto using gv_inject_incr.
-
+  split; auto.
     intros. apply J2 in H. 
     destruct H as [bv2 [ev2 [bgv2 [egv2 [H1 [H2 [H3 [H4 H5]]]]]]]].
     exists bv2. exists ev2. exists bgv2. exists egv2.
     repeat (split; eauto using gv_inject_incr).
-Qed.
-
-Lemma val_list_inject_app : forall mi vs1 vs1' vs2 vs2',
-  val_list_inject mi vs1 vs2 ->
-  val_list_inject mi vs1' vs2' ->
-  val_list_inject mi (vs1++vs1') (vs2++vs2').
-Proof.
-  induction vs1; destruct vs2; simpl; intros; inv H; auto.
-Qed.
-
-Lemma gv_inject_app : forall mi gv1 gv1' gv2 gv2',
-  gv_inject mi gv1 gv2 ->
-  gv_inject mi gv1' gv2' ->
-  gv_inject mi (gv1++gv1') (gv2++gv2').
-Proof.
-  unfold gv_inject.
-  induction gv1; destruct gv2; simpl; intros; auto.  
-    destruct p. destruct (split gv2). inv H.
-    destruct a. destruct (split gv1). inv H.
-
-    destruct a. remember (split gv1) as R3. destruct R3.
-    destruct p. remember (split gv2) as R4. destruct R4. 
-    inv H.
-    remember (split (gv1 ++ gv1')) as R1. destruct R1.
-    remember (split (gv2 ++ gv2')) as R2. destruct R2.
-    apply val_cons_inject; auto.
-      assert (J:=@IHgv1 gv1' gv2 gv2').
-      rewrite <- HeqR4 in J.
-      rewrite <- HeqR1 in J.
-      rewrite <- HeqR2 in J.
-      eapply J; eauto.
-Qed.
-
-Definition zeroconst2GV__gv_inject_refl_prop (t:typ) := 
-  forall maxb mi Mem1 Mem2 gv TD, 
-  wf_sb_mi maxb mi Mem1 Mem2 ->
-  zeroconst2GV TD t = Some gv ->
-  gv_inject mi gv gv.
-  
-Definition zeroconsts2GV__gv_inject_refl_prop (lt:list_typ) := 
-  forall maxb mi Mem1 Mem2 gv TD n, 
-  wf_sb_mi maxb mi Mem1 Mem2 ->
-  zeroconsts2GV TD lt = Some (gv,n) ->
-  gv_inject mi gv gv.
-
-Ltac tinv H := try solve [inv H].
-  
-Lemma gv_inject__repeatGV : forall mi gv1 gv2 n,
-  gv_inject mi gv1 gv2 -> 
-  gv_inject mi (repeatGV gv1 n) (repeatGV gv2 n).
-Proof.
-  induction n; intros.
-    unfold gv_inject. simpl. auto.
-    simpl. eapply gv_inject_app; eauto.
-Qed.
-
-Lemma gv_inject_uninits : forall mi n, gv_inject mi (uninits n) (uninits n).
-Proof.
-  unfold uninits.
-  induction n.
-    unfold gv_inject. simpl; auto.
-    simpl. simpl_env. apply gv_inject_app; auto.
-      unfold gv_inject. simpl; auto.
-Qed.
-
-Lemma zeroconst2GV__gv_inject_refl_mutrec :
-  (forall t, zeroconst2GV__gv_inject_refl_prop t) *
-  (forall lt, zeroconsts2GV__gv_inject_refl_prop lt).
-Proof.
-  apply typ_mutrec; 
-    unfold zeroconst2GV__gv_inject_refl_prop, 
-           zeroconsts2GV__gv_inject_refl_prop; 
-    intros; simpl in *; 
-    try solve [unfold gv_inject; simpl in *; eauto | 
-               inversion H0 | inversion H1 | inversion H2].
-
-  unfold gv_inject.
-  inv H0. simpl. 
-  apply val_cons_inject; auto.
-
-  unfold gv_inject.
-  destruct f; inv H0; simpl; apply val_cons_inject; auto.
-
-  remember (zeroconst2GV TD t) as R.
-  destruct R; tinv H1.
-  destruct (getTypeStoreSize TD t); tinv H1.
-  destruct (getTypeAllocSize TD t); inv H1.
-  simpl. symmetry in HeqR.
-  eapply H in HeqR; eauto.
-  apply gv_inject__repeatGV.
-  apply gv_inject_app; auto.
-    apply gv_inject_uninits.
-
-  remember (zeroconsts2GV TD l0) as R.
-  destruct R as [[gv0 tsz]|]; tinv H1.
-  destruct (getTypeAllocSize TD (typ_struct l0)); inv H1.
-  destruct l0; inv H3.
-    apply gv_inject_uninits.
-    symmetry in HeqR.
-    eapply H in HeqR; eauto.
-    apply gv_inject_app; auto.
-      apply gv_inject_uninits.
- 
-  inv H1. unfold gv_inject. simpl.
-  apply val_cons_inject; auto.
-    inv H0. 
-    eapply val_inject_ptr; eauto.
-
-  inv H0. unfold gv_inject. simpl. auto.
-
-
-  remember (zeroconsts2GV TD l0) as R.
-  destruct R as [[gv1 tsz]|]; tinv H2.
-  remember (zeroconst2GV TD t) as R1.
-  destruct R1 as [gv2|]; tinv H2.
-  destruct (getTypeStoreSize TD t); inv H2.
-  destruct (getTypeAllocSize TD t); inv H4.
-  symmetry in HeqR.
-  eapply H0 in HeqR; eauto.
-  symmetry in HeqR1.
-  eapply H in HeqR1; eauto.
-  apply gv_inject_app; auto.
-  apply gv_inject_app; auto.
-    apply gv_inject_uninits.
-Qed.
-
-Lemma zeroconst2GV__gv_inject_refl : forall maxb mi Mem1 Mem2 gv TD t, 
-  wf_sb_mi maxb mi Mem1 Mem2 ->
-  zeroconst2GV TD t = Some gv ->
-  gv_inject mi gv gv.
-Proof.
-  intros.  
-  destruct zeroconst2GV__gv_inject_refl_mutrec as [J _].
-  unfold zeroconst2GV__gv_inject_refl_prop in J.
-  eauto.
-Qed. 
-
-Lemma global_gv_inject_refl_aux : forall maxb mi Mem1 Mem2 gv,
-  wf_sb_mi maxb mi Mem1 Mem2 ->
-  wf_global maxb gv ->
-  gv_inject mi gv gv.
-Proof.
-  unfold gv_inject.
-  induction gv; intros; simpl; auto.
-    destruct a.
-    remember (split gv) as R.
-    destruct R.
-      destruct v; simpl in *; try solve 
-        [assert (J:=@IHgv H H0); eauto].
-
-        destruct H0 as [H1 H2].
-        assert (J:=(@IHgv H H2)).
-        inversion H.
-        apply mi_globals in H1.
-        apply val_cons_inject; auto.
-          apply val_inject_ptr with (delta:=0); auto.
-            rewrite Int.add_zero; auto.
-Qed.
-
-Lemma wf_globals__wf_global : forall mgb gl gv i0,
-  wf_globals mgb gl ->
-  ret gv = lookupAL GenericValue gl i0 ->
-  wf_global mgb gv.
-Proof.
-  induction gl; intros.
-    inversion H0.
-
-    destruct a. simpl in *.
-    destruct H as [J1 J2].
-    destruct (i0 == i1); subst; eauto.
-      inv H0; auto.
-Qed.      
-
-Lemma global_gv_inject_refl : forall maxb mi Mem1 Mem2 gl i0 gv,
-  wf_sb_mi maxb mi Mem1 Mem2 ->
-  wf_globals maxb gl ->
-  lookupAL _ gl i0 = Some gv ->
-  gv_inject mi gv gv.
-Proof.
-  intros. 
-  eapply global_gv_inject_refl_aux; eauto.
-    eapply wf_globals__wf_global; eauto.
-Qed.
-    
-Lemma gv_inject_nil_inv : forall mi gv2,
-  gv_inject mi nil gv2 -> gv2 = nil.
-Proof.
-  intros.   
-  destruct gv2; eauto.
-  unfold gv_inject in H. simpl in H. destruct p. destruct (split gv2). inv H.
-Qed.    
-
-Lemma gv_inject_nil_inv' : forall mi gv1,
-  gv_inject mi gv1 nil -> gv1 = nil.
-Proof.
-  intros.   
-  destruct gv1; eauto.
-  unfold gv_inject in H. simpl in H. destruct p. destruct (split gv1). inv H.
-Qed.    
-
-Lemma gv_inject_cons_inv : forall mi g1 gv1 gv2,
-  gv_inject mi (g1::gv1) gv2 -> 
-  exists gv2', exists v1, exists m1, exists v2, exists m2, 
-    gv2 = (v2,m2)::gv2' /\ gv_inject mi gv1 gv2' /\ val_inject mi v1 v2 /\
-    g1 = (v1,m1).
-Proof.
-  intros.   
-  destruct gv2; eauto.
-    apply gv_inject_nil_inv' in H. inv H.
-    unfold gv_inject in H. simpl in H. destruct g1. 
-    remember (split gv1) as R1.  destruct R1. destruct p.
-    remember (split gv2) as R2.  destruct R2. 
-    inv H. exists gv2. exists v. exists m. exists v0. exists m0.
-    unfold gv_inject. rewrite <- HeqR1. rewrite <- HeqR2.
-    split; auto.
-Qed.    
-
-Lemma gv_inject__val_inject : forall mi gv1 gv2 TD,
-  gv_inject mi gv1 gv2 ->
-  exists v1, exists v2,
-    GV2val TD gv1 = Some v1 /\ GV2val TD gv2 = Some v2 /\ val_inject mi v1 v2.
-Proof.
-  intros.
-  unfold GV2val in *.
-  destruct gv1.
-    apply gv_inject_nil_inv in H. subst. eauto.
-
-    apply gv_inject_cons_inv in H.
-    destruct H as [gv2' [v1' [m1 [v2 [m2 [J1 [J2 [J3 J4]]]]]]]]; subst.
-    destruct gv1.
-      apply gv_inject_nil_inv in J2. subst. eauto.
-  
-      apply gv_inject_cons_inv in J2.
-      destruct J2 as [gv3 [v2' [m2' [v3 [m3 [J1 [J2 [J5 J4]]]]]]]]; subst.
-      eauto.
-Qed.
-
-Lemma gv_inject_gundef : forall mi, gv_inject mi gundef gundef.
-Proof.
-  intros. unfold gundef. apply gv_inject_uninits.
-Qed.
-
-Lemma simulation__mtrunc_aux : forall mi TD top t1 gv1 t2 gv1' gv2,
-  gv_inject mi gv1 gv1' ->
-  mtrunc TD top t1 gv1 t2 = Some gv2 ->
-  (mtrunc TD top t1 gv1 t2 = mtrunc TD top t1 gv1' t2 /\
-    gv_inject mi gv2 gv2) \/
-  exists gv2',
-    mtrunc TD top t1 gv1' t2 = Some gv2' /\
-    gv_inject mi gv2 gv2'.  
-Proof.
-  intros.
-  apply gv_inject__val_inject with (TD:=TD) in H.
-  destruct H as [v1 [v2 [J1 [J2 J3]]]].
-  unfold mtrunc in *.
-  rewrite J1. rewrite J2. rewrite J1 in H0. unfold gv_inject.
-  inv J3; auto.
-    destruct t1; destruct t2; inv H0; simpl; auto.
-      destruct (le_lt_dec wz s0); auto.
-    destruct t1; destruct t2; inv H0; simpl; auto.
-      destruct (floating_point_order f1 f0); inv H1; simpl; auto.
-      destruct f1; inv H0; simpl; auto.
-    inv H0. simpl. auto.
-    inv H0. simpl. auto.
-
-    right. inv H0.
-    destruct v2; try solve [exists gundef; simpl; auto using gv_inject_gundef].
-      destruct t1; try solve [exists gundef; simpl; auto using gv_inject_gundef].
-      destruct t2; try solve [exists gundef; simpl; auto using gv_inject_gundef].
-        exists (val2GV TD (Val.trunc (Vint wz i0) s0) (AST.Mint s0)).
-        split; auto.  
-          unfold val2GV, gv_inject. simpl.
-          destruct (le_lt_dec wz s0); auto.
-
-      destruct t1; try solve [exists gundef; simpl; auto using gv_inject_gundef].
-      destruct t2; try solve [exists gundef; simpl; auto using gv_inject_gundef].
-      destruct (floating_point_order f1 f0);
-        try solve [exists gundef; simpl; auto using gv_inject_gundef].
-      destruct f1; try solve [exists gundef; simpl; auto using gv_inject_gundef].
-        exists (val2GV TD (Val.ftrunc (Vfloat f)) AST.Mfloat32).
-          simpl. auto.  
-        exists (val2GV TD (Val.ftrunc (Vfloat f)) AST.Mfloat64).
-          simpl. auto.  
-Qed.
-
-Lemma simulation__mtrunc : forall mi TD top t1 gv1 t2 gv1' gv2,
-  gv_inject mi gv1 gv1' ->
-  mtrunc TD top t1 gv1 t2 = Some gv2 ->
-  exists gv2',
-    mtrunc TD top t1 gv1' t2 = Some gv2' /\
-    gv_inject mi gv2 gv2'.
-Proof.
-  intros.
-  assert (J:=H0).
-  eapply simulation__mtrunc_aux in H0; eauto.
-  destruct H0 as [[H1 H2] | H0]; eauto.
-    rewrite <- H1.
-    exists gv2. split; auto.
-Qed.
-
-Lemma simulation__mext_aux : forall mi TD eop t1 gv1 t2 gv1' gv2,
-  gv_inject mi gv1 gv1' ->
-  mext TD eop t1 gv1 t2 = Some gv2 ->
-  (mext TD eop t1 gv1 t2 = mext TD eop t1 gv1' t2 /\
-    gv_inject mi gv2 gv2) \/
-  exists gv2',
-    mext TD eop t1 gv1' t2 = Some gv2' /\
-    gv_inject mi gv2 gv2'.  
-Proof.
-  intros. assert (J0:=H).
-  apply gv_inject__val_inject with (TD:=TD) in H.
-  destruct H as [v1 [v2 [J1 [J2 J3]]]].
-  unfold mext in *.
-  rewrite J1. rewrite J2. rewrite J1 in H0. unfold gv_inject.
-  inv J3; auto.
-    destruct t1; destruct t2; inv H0; simpl; auto.
-      destruct eop; inv H1; simpl; auto.
-      destruct (floating_point_order f f0); inv H1; simpl; auto.
-
-    destruct t1; destruct t2; inv H0; simpl; auto.
-      destruct (floating_point_order f0 f1); inv H1; simpl; auto.
-      destruct eop; inv H0; simpl; auto.
-      right. exists gv1'. split; auto.        
-
-    destruct t1; destruct t2; inv H0; simpl; auto.
-      destruct (floating_point_order f f0); inv H2; simpl; auto.
-
-    destruct t1; destruct t2; inv H0; simpl; auto.
-      destruct (floating_point_order f f0); inv H1; simpl; auto.
-
-    destruct t1; destruct t2; inv H0; simpl; auto.
-      destruct v2; simpl; auto.
-      destruct eop; auto.
-        right. exists (val2GV TD (Vint wz (Int.zero_ext wz (Size.to_Z s0) i0))
-           (AST.Mint (Size.to_nat s0 - 1))).
-        simpl. auto.
-        right. exists (val2GV TD (Vint wz (Int.sign_ext wz (Size.to_Z s0) i0))
-            (AST.Mint (Size.to_nat s0 - 1))).
-        simpl. auto.
-      destruct (floating_point_order f f0); inv H1; simpl; eauto.
-        destruct v2; simpl; auto.
-        destruct eop; simpl; auto.
-          right. exists gv1'. split; auto.
-          destruct gv1'; inv J2.
-          destruct p.
-          destruct gv1'; inv H0.
-          simpl. auto.
-Qed.
-
-Lemma simulation__mext : forall mi TD eop t1 gv1 t2 gv1' gv2,
-  gv_inject mi gv1 gv1' ->
-  mext TD eop t1 gv1 t2 = Some gv2 ->
-  exists gv2',
-    mext TD eop t1 gv1' t2 = Some gv2' /\
-    gv_inject mi gv2 gv2'.
-Proof.
-  intros.
-  assert (J:=H0).
-  eapply simulation__mext_aux in H0; eauto.
-  destruct H0 as [[H1 H2] | H0]; eauto.
-    rewrite <- H1.
-    exists gv2. split; auto.
-Qed.
-
-Lemma add_isnt_ptr : forall wz i0 wz0 i1 b ofs,
-  Val.add (Vint wz i0) (Vint wz0 i1) <> Vptr b ofs.
-Proof.
-  intros.
-  Val.simpl_add; try congruence.
-    unfold Val.add_obligation_1. 
-    unfold DepElim.solution_left.
-    unfold eq_rect_r. simpl. congruence.
-Qed.
-
-Lemma sub_isnt_ptr : forall wz i0 wz0 i1 b ofs,
-  Val.sub (Vint wz i0) (Vint wz0 i1) <> Vptr b ofs.
-Proof.
-  intros.
-  Val.simpl_sub; try congruence.
-    unfold Val.sub_obligation_1. 
-    unfold DepElim.solution_left.
-    unfold eq_rect_r. simpl. congruence.
-Qed.
-
-Lemma mul_isnt_ptr : forall wz i0 wz0 i1 b ofs,
-  Val.mul (Vint wz i0) (Vint wz0 i1) <> Vptr b ofs.
-Proof.
-  intros.
-  Val.simpl_mul; try congruence.
-    unfold Val.mul_obligation_1. 
-    unfold DepElim.solution_left.
-    unfold eq_rect_r. simpl. congruence.
-Qed.
-
-Lemma divu_isnt_ptr : forall wz i0 wz0 i1 b ofs,
-  Val.divu (Vint wz i0) (Vint wz0 i1) <> Vptr b ofs.
-Proof.
-  intros.
-  Val.simpl_divu; try congruence.
-    unfold Val.divu_obligation_1. 
-    unfold DepElim.solution_left.
-    unfold eq_rect_r. simpl. 
-    destruct (Int.eq wz0 i1 (Int.zero wz0)); congruence.
-Qed.
-
-Lemma divs_isnt_ptr : forall wz i0 wz0 i1 b ofs,
-  Val.divs (Vint wz i0) (Vint wz0 i1) <> Vptr b ofs.
-Proof.
-  intros.
-  Val.simpl_divs; try congruence.
-    unfold Val.divs_obligation_1. 
-    unfold DepElim.solution_left.
-    unfold eq_rect_r. simpl. 
-    destruct (Int.eq wz0 i1 (Int.zero wz0)); congruence.
-Qed.
-
-Lemma modu_isnt_ptr : forall wz i0 wz0 i1 b ofs,
-  Val.modu (Vint wz i0) (Vint wz0 i1) <> Vptr b ofs.
-Proof.
-  intros.
-  Val.simpl_modu; try congruence.
-    unfold Val.modu_obligation_1. 
-    unfold DepElim.solution_left.
-    unfold eq_rect_r. simpl. 
-    destruct (Int.eq wz0 i1 (Int.zero wz0)); congruence.
-Qed.
-
-Lemma mods_isnt_ptr : forall wz i0 wz0 i1 b ofs,
-  Val.mods (Vint wz i0) (Vint wz0 i1) <> Vptr b ofs.
-Proof.
-  intros.
-  Val.simpl_mods; try congruence.
-    unfold Val.mods_obligation_1. 
-    unfold DepElim.solution_left.
-    unfold eq_rect_r. simpl. 
-    destruct (Int.eq wz0 i1 (Int.zero wz0)); congruence.
-Qed.
-
-Lemma shl_isnt_ptr : forall wz i0 wz0 i1 b ofs,
-  Val.shl (Vint wz i0) (Vint wz0 i1) <> Vptr b ofs.
-Proof.
-  intros.
-  Val.simpl_shl; try congruence.
-    unfold Val.shl_obligation_1. 
-    unfold DepElim.solution_left.
-    unfold eq_rect_r. simpl. 
-    destruct (Int.ltu wz0 i1 (Int.iwordsize wz0)); congruence.
-Qed.
-
-Lemma shrx_isnt_ptr : forall wz i0 wz0 i1 b ofs,
-  Val.shrx (Vint wz i0) (Vint wz0 i1) <> Vptr b ofs.
-Proof.
-  intros.
-  Val.simpl_shrx; try congruence.
-    unfold Val.shrx_obligation_1. 
-    unfold DepElim.solution_left.
-    unfold eq_rect_r. simpl. 
-    destruct (Int.ltu wz0 i1 (Int.iwordsize wz0)); congruence.
-Qed.
-
-Lemma shr_isnt_ptr : forall wz i0 wz0 i1 b ofs,
-  Val.shr (Vint wz i0) (Vint wz0 i1) <> Vptr b ofs.
-Proof.
-  intros.
-  Val.simpl_shr; try congruence.
-    unfold Val.shr_obligation_1. 
-    unfold DepElim.solution_left.
-    unfold eq_rect_r. simpl. 
-    destruct (Int.ltu wz0 i1 (Int.iwordsize wz0)); congruence.
-Qed.
-
-Lemma and_isnt_ptr : forall wz i0 wz0 i1 b ofs,
-  Val.and (Vint wz i0) (Vint wz0 i1) <> Vptr b ofs.
-Proof.
-  intros.
-  Val.simpl_and; try congruence.
-    unfold Val.and_obligation_1. 
-    unfold DepElim.solution_left.
-    unfold eq_rect_r. simpl. 
-    congruence.
-Qed.
-
-Lemma or_isnt_ptr : forall wz i0 wz0 i1 b ofs,
-  Val.or (Vint wz i0) (Vint wz0 i1) <> Vptr b ofs.
-Proof.
-  intros.
-  Val.simpl_or; try congruence.
-    unfold Val.or_obligation_1. 
-    unfold DepElim.solution_left.
-    unfold eq_rect_r. simpl. 
-    congruence.
-Qed.
-
-Lemma xor_isnt_ptr : forall wz i0 wz0 i1 b ofs,
-  Val.xor (Vint wz i0) (Vint wz0 i1) <> Vptr b ofs.
-Proof.
-  intros.
-  Val.simpl_xor; try congruence.
-    unfold Val.xor_obligation_1. 
-    unfold DepElim.solution_left.
-    unfold eq_rect_r. simpl. 
-    congruence.
-Qed.
-
-Lemma gv_inject_nptr_val_refl : forall TD v mi m,
-  (forall b ofs, v <> Vptr b ofs) ->
-  gv_inject mi (val2GV TD v m) (val2GV TD v m).
-Proof.
-  intros. unfold val2GV, gv_inject. simpl.
-  destruct v; auto. 
-    assert (J:=@H b i0). contradict J; auto.
-Qed.
-
-Lemma gv_inject_gundef_any_val : forall TD v mi m,
-  gv_inject mi gundef (val2GV TD v m).
-Proof.
-  intros. unfold val2GV, gv_inject. simpl.
-  destruct v; auto. 
-Qed.
-
-Lemma simulation__mbop_aux : forall mi TD op bsz gv1 gv1' gv2 gv2' gv3,
-  gv_inject mi gv1 gv1' ->
-  gv_inject mi gv2 gv2' ->
-  mbop TD op bsz gv1 gv2 = Some gv3 ->
-  (mbop TD op bsz gv1 gv2 = mbop TD op bsz gv1' gv2' /\
-    gv_inject mi gv3 gv3) \/
-  exists gv3',
-    mbop TD op bsz gv1' gv2' = Some gv3' /\
-    gv_inject mi gv3 gv3'.  
-Proof.
-  intros. assert (J0:=H0). assert (J:=H).
-  apply gv_inject__val_inject with (TD:=TD) in H.
-  destruct H as [v1 [v1' [J1 [J2 J3]]]].
-  apply gv_inject__val_inject with (TD:=TD) in H0.
-  destruct H0 as [v2 [v2' [J1' [J2' J3']]]].
-  unfold mbop in *.
-  rewrite J1. rewrite J2. rewrite J1'. rewrite J2'.  
-  rewrite J1 in H1. rewrite J1' in H1. 
-  inv J3; try solve [inv H1; auto using gv_inject_gundef].
-    inv J3'; try solve [auto | inv H1; auto using gv_inject_gundef].
-    destruct (eq_nat_dec (wz + 1) (Size.to_nat bsz)); 
-       try solve [inv H1; auto using gv_inject_gundef].
-    destruct op; inv H1; 
-       try (left; split; auto; apply gv_inject_nptr_val_refl; auto).
-       apply add_isnt_ptr.
-       apply sub_isnt_ptr.
-       apply mul_isnt_ptr.
-       apply divu_isnt_ptr.
-       apply divs_isnt_ptr.
-       apply modu_isnt_ptr.
-       apply mods_isnt_ptr.
-       apply shl_isnt_ptr.
-       apply shrx_isnt_ptr.
-       apply shr_isnt_ptr.
-       apply and_isnt_ptr.
-       apply or_isnt_ptr.
-       apply xor_isnt_ptr.
-
-    inv H1.
-      destruct v2'; auto using gv_inject_gundef.
-      destruct (eq_nat_dec (wz + 1) (Size.to_nat bsz)); 
-        auto using gv_inject_gundef.
-      destruct op; try solve [right; eauto using gv_inject_gundef_any_val].
-
-    inv H1.
-      destruct v1'; try solve [auto using gv_inject_gundef].
-      destruct v2'; try solve [auto using gv_inject_gundef].
-      destruct (eq_nat_dec (wz + 1) (Size.to_nat bsz)); 
-        auto using gv_inject_gundef.
-      destruct op; try solve [right; eauto using gv_inject_gundef_any_val].
-Qed.
-
-Lemma simulation__mbop : forall mi TD op bsz gv1 gv1' gv2 gv2' gv3,
-  gv_inject mi gv1 gv1' ->
-  gv_inject mi gv2 gv2' ->
-  mbop TD op bsz gv1 gv2 = Some gv3 ->
-  exists gv3',
-    mbop TD op bsz gv1' gv2' = Some gv3' /\
-    gv_inject mi gv3 gv3'.
-Proof.
-  intros.
-  assert (J:=H1).
-  eapply simulation__mbop_aux in H1; eauto.
-  destruct H1 as [[H1 H2] | H1]; eauto.
-    rewrite <- H1.
-    exists gv3. split; auto.
-Qed.
-
-Lemma simulation__mfbop_aux : forall mi TD op fp gv1 gv1' gv2 gv2' gv3,
-  gv_inject mi gv1 gv1' ->
-  gv_inject mi gv2 gv2' ->
-  mfbop TD op fp gv1 gv2 = Some gv3 ->
-  (mfbop TD op fp gv1 gv2 = mfbop TD op fp gv1' gv2' /\
-    gv_inject mi gv3 gv3) \/
-  exists gv3',
-    mfbop TD op fp gv1' gv2' = Some gv3' /\
-    gv_inject mi gv3 gv3'.  
-Proof.
-  intros. assert (J0:=H0). assert (J:=H).
-  apply gv_inject__val_inject with (TD:=TD) in H.
-  destruct H as [v1 [v1' [J1 [J2 J3]]]].
-  apply gv_inject__val_inject with (TD:=TD) in H0.
-  destruct H0 as [v2 [v2' [J1' [J2' J3']]]].
-  unfold mfbop in *.
-  rewrite J1. rewrite J2. rewrite J1'. rewrite J2'.  
-  rewrite J1 in H1. rewrite J1' in H1. 
-  inv J3; try solve [inv H1; auto using gv_inject_gundef].
-    inv J3'; try solve [auto | inv H1; auto using gv_inject_gundef].
-    destruct fp; inv H1; try solve [auto using gv_inject_gundef].
-       destruct op; 
-          try (left; split; auto; apply gv_inject_nptr_val_refl; 
-            try solve [auto | intro; congruence]).
-       destruct op; 
-          try (left; split; auto; apply gv_inject_nptr_val_refl; 
-            try solve [auto | intro; congruence]).
-
-   inv H1. 
-   destruct v2'; auto using gv_inject_gundef.
-   destruct fp; try solve [
-     destruct op; try solve [right; eauto using gv_inject_gundef_any_val] |
-     auto using gv_inject_gundef
-     ].
-
-   destruct v1'; auto using gv_inject_gundef.
-      inv H1. auto using gv_inject_gundef.
-      inv H1. auto using gv_inject_gundef.
-      inv H1. auto using gv_inject_gundef.
-      destruct v2'; auto using gv_inject_gundef.
-
-   destruct fp; try solve [ 
-      destruct op; try solve [right; eauto using gv_inject_gundef_any_val] |
-      auto using gv_inject_gundef |
-      inv H1; auto using gv_inject_gundef
-     ].
-   inv H1. auto using gv_inject_gundef.
-   inv H1. auto using gv_inject_gundef.
-Qed.
-
-Lemma simulation__mfbop : forall mi TD op fp gv1 gv1' gv2 gv2' gv3,
-  gv_inject mi gv1 gv1' ->
-  gv_inject mi gv2 gv2' ->
-  mfbop TD op fp gv1 gv2 = Some gv3 ->
-  exists gv3',
-    mfbop TD op fp gv1' gv2' = Some gv3' /\
-    gv_inject mi gv3 gv3'.
-Proof.
-  intros.
-  assert (J:=H1).
-  eapply simulation__mfbop_aux in H1; eauto.
-  destruct H1 as [[H1 H2] | H1]; eauto.
-    rewrite <- H1.
-    exists gv3. split; auto.
-Qed.
-
-Lemma simulation__mcast_aux_helper : forall TD gv1' wz i0 mi gv2
-  (J2 : GV2val TD gv1' = ret Vint wz i0)
-  (J : gv_inject mi gv2 gv1')
-  (J1 : GV2val TD gv2 = ret Vint wz i0),
-   ret gv2 = ret gv1' /\ gv_inject mi gv2 gv2 \/
-   (exists gv2' : GenericValue, ret gv1' = ret gv2' /\ gv_inject mi gv2 gv2').
-Proof. intros.
-        unfold GV2val in *.
-        destruct gv1'; tinv J2.
-        destruct p; tinv J2.
-        destruct gv1'; tinv J2.
-        destruct gv2; tinv J1.
-        destruct p; tinv J1.
-        destruct gv2; inv J1.
-        right. exists ((v, m) :: nil). 
-        unfold gv_inject. simpl. auto.
-Qed.
-
-Lemma simulation__mcast_aux : forall mi TD op t1 t2 gv1 gv1' gv2,
-  gv_inject mi gv1 gv1' ->
-  mcast TD op t1 gv1 t2 = Some gv2 ->
-  (mcast TD op t1 gv1 t2 = mcast TD op t1 gv1' t2 /\
-    gv_inject mi gv2 gv2) \/
-  exists gv2',
-    mcast TD op t1 gv1' t2 = Some gv2' /\
-    gv_inject mi gv2 gv2'.  
-Proof.
-  intros.  assert (J:=H).
-  apply gv_inject__val_inject with (TD:=TD) in H.
-  destruct H as [v1 [v1' [J1 [J2 J3]]]].
-  unfold mcast, mbitcast in *.
-  inv J3; try solve [
-    destruct op; try solve [
-      destruct t1; try solve [
-        inv H0 |
-        destruct t2; inv H0; [eauto using simulation__mcast_aux_helper]
-      ] |
-      destruct t1; try solve [
-        inv H0 |
-        destruct t2; inv H0; [auto using gv_inject_gundef] 
-      ]
-    ]
-  ].
-Qed.
-
-Lemma simulation__mcast : forall mi TD op t1 gv1 gv1' t2 gv2,
-  gv_inject mi gv1 gv1' ->
-  mcast TD op t1 gv1 t2 = Some gv2 ->
-  exists gv2',
-    mcast TD op t1 gv1' t2 = Some gv2' /\
-    gv_inject mi gv2 gv2'.
-Proof.
-  intros.
-  assert (J:=H0).
-  eapply simulation__mcast_aux in H0; eauto.
-  destruct H0 as [[H1 H2] | H1]; eauto.
-    rewrite <- H1.
-    exists gv2. split; auto.
-Qed.
-
-
-Lemma cmp_isnt_ptr : forall c wz i0 wz0 i1 b ofs,
-  Val.cmp c (Vint wz i0) (Vint wz0 i1) <> Vptr b ofs.
-Proof.
-  intros.
-  Val.simpl_cmp; try congruence.
-    unfold Val.cmp_obligation_1. 
-    unfold DepElim.solution_left.
-    unfold eq_rect_r. simpl. 
-    unfold Val.of_bool.
-    destruct (Int.cmp wz0 c i0 i1).
-      unfold Vtrue. unfold Vone. congruence.
-      unfold Vfalse. unfold Vzero. congruence.
-Qed.
-
-Lemma cmpu_isnt_ptr : forall c wz i0 wz0 i1 b ofs,
-  Val.cmpu c (Vint wz i0) (Vint wz0 i1) <> Vptr b ofs.
-Proof.
-  intros.
-  Val.simpl_cmpu; try congruence.
-    unfold Val.cmpu_obligation_1. 
-    unfold DepElim.solution_left.
-    unfold eq_rect_r. simpl. 
-    unfold Val.of_bool.
-    destruct (Int.cmpu wz0 c i0 i1).
-      unfold Vtrue. unfold Vone. congruence.
-      unfold Vfalse. unfold Vzero. congruence.
-Qed.
-
-Lemma simulation__micmp_aux : forall mi TD c t gv1 gv1' gv2 gv2' gv3,
-  gv_inject mi gv1 gv1' ->
-  gv_inject mi gv2 gv2' ->
-  micmp TD c t gv1 gv2 = Some gv3 ->
-  (micmp TD c t gv1 gv2 = micmp TD c t gv1' gv2' /\
-    gv_inject mi gv3 gv3) \/
-  exists gv3',
-    micmp TD c t gv1' gv2' = Some gv3' /\
-    gv_inject mi gv3 gv3'.  
-Proof.
-  intros. assert (J0:=H0). assert (J:=H).
-  apply gv_inject__val_inject with (TD:=TD) in H.
-  destruct H as [v1 [v1' [J1 [J2 J3]]]].
-  apply gv_inject__val_inject with (TD:=TD) in H0.
-  destruct H0 as [v2 [v2' [J1' [J2' J3']]]].
-  unfold micmp, micmp_int in *.
-  rewrite J1. rewrite J2. rewrite J1'. rewrite J2'.  
-  rewrite J1 in H1. rewrite J1' in H1. 
-  inv J3; try solve [inv H1; auto using gv_inject_gundef].
-    inv J3'; try solve [auto | inv H1; auto using gv_inject_gundef];
-    destruct t; try solve [inv H1; auto using gv_inject_gundef].
-      destruct c; inv H1; 
-        try (left; split; auto; 
-          apply gv_inject_nptr_val_refl; try solve 
-            [auto | apply cmp_isnt_ptr | apply cmpu_isnt_ptr]).
-    inv H1.
-     destruct v2'; try solve [auto using gv_inject_gundef].
-     destruct c; try solve [right; eauto using gv_inject_gundef_any_val].
-    destruct t; try solve [inv H1; auto using gv_inject_gundef].
-    destruct t; try solve [inv H1; auto using gv_inject_gundef].
-    destruct t; try solve [inv H1; auto using gv_inject_gundef].
-    destruct t; try solve [inv H1; auto using gv_inject_gundef].
-    inv H1.
-     destruct v1'; try solve [auto using gv_inject_gundef].
-     destruct v2'; try solve [auto using gv_inject_gundef].
-     destruct c; try solve [right; eauto using gv_inject_gundef_any_val].
-Qed.
-
-Lemma simulation__micmp : forall mi TD c t gv1 gv1' gv2 gv2' gv3,
-  gv_inject mi gv1 gv1' ->
-  gv_inject mi gv2 gv2' ->
-  micmp TD c t gv1 gv2 = Some gv3 ->
-  exists gv3',
-    micmp TD c t gv1' gv2' = Some gv3' /\
-    gv_inject mi gv3 gv3'.
-Proof.
-  intros.
-  assert (J:=H1).
-  eapply simulation__micmp_aux in H1; eauto.
-  destruct H1 as [[H1 H2] | H1]; eauto.
-    rewrite <- H1.
-    exists gv3. split; auto.
-Qed.
-
-Lemma val_of_bool_isnt_ptr : forall v b ofs,
-  Val.of_bool v <> Vptr b ofs.
-Proof.
-  intros. unfold Val.of_bool. destruct v. 
-    unfold Vtrue. unfold Vone. congruence.
-    unfold Vfalse. unfold Vzero. congruence.
-Qed.
-
-Lemma Vfalse_isnt_ptr : forall b ofs,
-  Vfalse <> Vptr b ofs.
-Proof.
-  intros. unfold Vfalse. unfold Vzero. congruence.
-Qed.
-
-Lemma Vtrue_isnt_ptr : forall b ofs,
-  Vtrue <> Vptr b ofs.
-Proof.
-  intros. unfold Vtrue. unfold Vone. congruence.
-Qed.
-
-Lemma simulation__mfcmp_aux : forall mi TD c t gv1 gv1' gv2 gv2' gv3,
-  gv_inject mi gv1 gv1' ->
-  gv_inject mi gv2 gv2' ->
-  mfcmp TD c t gv1 gv2 = Some gv3 ->
-  (mfcmp TD c t gv1 gv2 = mfcmp TD c t gv1' gv2' /\
-    gv_inject mi gv3 gv3) \/
-  exists gv3',
-    mfcmp TD c t gv1' gv2' = Some gv3' /\
-    gv_inject mi gv3 gv3'.  
-Proof.
-  intros. assert (J0:=H0). assert (J:=H).
-  apply gv_inject__val_inject with (TD:=TD) in H.
-  destruct H as [v1 [v1' [J1 [J2 J3]]]].
-  apply gv_inject__val_inject with (TD:=TD) in H0.
-  destruct H0 as [v2 [v2' [J1' [J2' J3']]]].
-  unfold mfcmp in *.
-  rewrite J1. rewrite J2. rewrite J1'. rewrite J2'.  
-  rewrite J1 in H1. rewrite J1' in H1. 
-  inv J3; try solve [inv H1; auto using gv_inject_gundef].
-    inv J3'; try solve [auto | inv H1; auto using gv_inject_gundef];
-    destruct t; try solve [inv H1; auto using gv_inject_gundef].
-      destruct c; inv H1; 
-        try solve [
-          auto using gv_inject_gundef |
-          (left; split; auto; 
-          apply gv_inject_nptr_val_refl; try solve 
-            [auto | apply val_of_bool_isnt_ptr | apply Vfalse_isnt_ptr | 
-             apply Vtrue_isnt_ptr])
-        ].
-      destruct c; inv H1; 
-        try solve [
-          auto using gv_inject_gundef |
-          (left; split; auto; 
-          apply gv_inject_nptr_val_refl; try solve 
-            [auto | apply val_of_bool_isnt_ptr | apply Vfalse_isnt_ptr | 
-             apply Vtrue_isnt_ptr])
-        ].
-
-
-    inv H1.
-     destruct v2'; try solve [auto using gv_inject_gundef].
-     destruct c; try solve [
-       right; eauto using gv_inject_gundef_any_val |
-       auto using gv_inject_gundef
-     ].
-    inv H1.
-     destruct v2'; try solve [auto using gv_inject_gundef].
-     destruct c; try solve [
-       right; eauto using gv_inject_gundef_any_val |
-       auto using gv_inject_gundef
-     ].
-    inv H1. destruct v2'; try solve [auto using gv_inject_gundef].
-    inv H1. destruct v2'; try solve [auto using gv_inject_gundef].
-    inv H1. destruct v2'; try solve [auto using gv_inject_gundef].
-    inv H1.
-     destruct v1'; try solve [auto using gv_inject_gundef].
-     destruct v2'; try solve [auto using gv_inject_gundef].
-     destruct t; try solve [auto using gv_inject_gundef].
-       destruct c; try solve [auto using gv_inject_gundef |
-         right; eauto using gv_inject_gundef_any_val].
-       destruct c; try solve [auto using gv_inject_gundef |
-         right; eauto using gv_inject_gundef_any_val].
-Qed.
-
-Lemma simulation__mfcmp : forall mi TD c t gv1 gv1' gv2 gv2' gv3,
-  gv_inject mi gv1 gv1' ->
-  gv_inject mi gv2 gv2' ->
-  mfcmp TD c t gv1 gv2 = Some gv3 ->
-  exists gv3',
-    mfcmp TD c t gv1' gv2' = Some gv3' /\
-    gv_inject mi gv3 gv3'.
-Proof.
-  intros.
-  assert (J:=H1).
-  eapply simulation__mfcmp_aux in H1; eauto.
-  destruct H1 as [[H1 H2] | H1]; eauto.
-    rewrite <- H1.
-    exists gv3. split; auto.
-Qed.
-
-Lemma simulation__GV2ptr : forall mi TD gv1 gv1' v,
-  gv_inject mi gv1 gv1' ->
-  GV2ptr TD (getPointerSize TD) gv1 = Some v ->
-  exists v',
-    GV2ptr TD (getPointerSize TD) gv1' = Some v' /\
-    Values.val_inject mi v v'.
-Proof.
-  intros.
-  unfold GV2ptr in *.
-  destruct gv1; tinv H0.
-  destruct p; tinv H0.
-  destruct v0; tinv H0.
-  destruct gv1; inv H0.
-  unfold gv_inject in H.
-  destruct gv1'; tinv H.
-  destruct p; tinv H.
-  destruct gv1'; tinv H.
-    destruct v; simpl in H; inv H; inv H3. eauto.
-    destruct p. simpl in H. destruct (split gv1'). inv H. inv H5.
-Qed.
-
-Lemma simulation__mgep : forall mi TD v v' v0 t0 l1,
-  Values.val_inject mi v v' ->
-  mgep TD t0 v l1 = Some v0 ->
-  exists v0',
-    mgep TD t0 v' l1 = Some v0' /\
-    Values.val_inject mi v0 v0'.
-Proof.
-  intros.
-  unfold mgep in *.
-  destruct v; tinv H0.
-  destruct l1; tinv H0.
-  inv H.
-  destruct (mgetoffset TD (typ_array 0%nat t0) (z :: l1)); tinv H0.
-  inv H0. 
-  exists (Vptr b2 (Int.add 31 (Int.add 31 i0 (Int.repr 31 delta)) i1)).
-  split; auto.
-    eapply val_inject_ptr; eauto.
-      rewrite Int.add_assoc.
-      assert (Int.add 31 (Int.repr 31 delta) i1 = 
-              Int.add 31 i1 (Int.repr 31 delta)) as EQ.
-        rewrite Int.add_commut. auto.
-      rewrite EQ.
-      rewrite Int.add_assoc. auto.
-Qed.
-   
-Lemma gv_inject_nil_refl : forall mi, gv_inject mi nil nil.
-Proof.
-  intros. unfold gv_inject. simpl. auto.
-Qed.
-
-Lemma gv_inject_cons_intro : forall mi v1 m1 v2 m2 gv1 gv2,
-  gv_inject mi gv1 gv2 ->
-  val_inject mi v1 v2 ->
-  gv_inject mi ((v1, m1) :: gv1) ((v2, m2) :: gv2).
-Proof.
-  intros.
-  unfold gv_inject in *. simpl.
-  remember (split gv1) as R1.
-  remember (split gv2) as R2.
-  destruct R1. destruct R2.
-  eauto.
-Qed.  
-
-Lemma chunk_matched_nil_inv : forall gv2,
-  chunk_matched nil gv2 -> gv2 = nil.
-Proof.
-  intros.   
-  destruct gv2; eauto.
-  unfold chunk_matched in H. simpl in H. destruct p. destruct (split gv2). inv H.
-Qed.    
-
-Lemma chunk_matched_nil_inv' : forall gv1,
-  chunk_matched gv1 nil -> gv1 = nil.
-Proof.
-  intros.   
-  destruct gv1; eauto.
-  unfold chunk_matched in H. simpl in H. destruct p. destruct (split gv1). inv H.
-Qed.    
-
-Lemma chunk_matched_nil_refl : chunk_matched nil nil.
-Proof.
-  intros. unfold chunk_matched. simpl. auto.
-Qed.
-
-Lemma chunk_matched_cons_intro : forall v1 m v2 gv1 gv2,
-  chunk_matched gv1 gv2 ->
-  chunk_matched ((v1, m) :: gv1) ((v2, m) :: gv2).
-Proof.
-  intros.
-  unfold chunk_matched in *. simpl.
-  remember (split gv1) as R1.
-  remember (split gv2) as R2.
-  destruct R1. destruct R2.
-  inv H. auto.
-Qed.  
-
-Lemma chunk_matched_cons_inv : forall g1 gv1 gv2,
-  chunk_matched (g1::gv1) gv2 -> 
-  exists gv2', exists v1, exists m1, exists v2,
-    gv2 = (v2,m1)::gv2' /\ chunk_matched gv1 gv2' /\ g1 = (v1,m1).
-Proof.
-  intros.   
-  destruct gv2; eauto.
-    apply chunk_matched_nil_inv' in H. inv H.
-    unfold chunk_matched in H. simpl in H. destruct g1. 
-    remember (split gv1) as R1.  destruct R1. destruct p.
-    remember (split gv2) as R2.  destruct R2. 
-    inv H. exists gv2. exists v. exists m0. exists v0.
-    unfold chunk_matched. rewrite <- HeqR1. rewrite <- HeqR2.
-    split; auto.
-Qed.    
-
-Lemma simulation__splitGenericValue_some : forall mi gv gv' z gvl gvr,
-  chunk_matched gv gv' ->
-  gv_inject mi gv gv' ->
-  splitGenericValue gv z = Some (gvl, gvr) ->
-  exists gvl', exists gvr', 
-    splitGenericValue gv' z = Some (gvl', gvr') /\
-    gv_inject mi gvl gvl' /\ chunk_matched gvl gvl' /\
-    gv_inject mi gvr gvr' /\ chunk_matched gvr gvr'.
-Proof.
-  induction gv; simpl; intros gv' z gvl gvr J H H0.
-    apply gv_inject_nil_inv in H. subst.
-    simpl.
-    destruct (zeq z 0); inv H0. 
-      exists nil. exists nil. split; auto using gv_inject_nil_refl.
-      destruct (zlt z 0); inv H1.
-
-    apply gv_inject_cons_inv in H. 
-    destruct H as [gv2' [v1 [m1 [v2 [m2 [J1 [J2 [J3 J4]]]]]]]]; subst.
-    simpl.
-    destruct (zeq z 0); inv H0. 
-      exists nil. exists ((v2, m2)::gv2'). 
-      split; auto using gv_inject_nil_refl, gv_inject_cons_intro,
-         chunk_matched_nil_refl, chunk_matched_cons_intro.
-    destruct (zlt z 0); inv H1.
-    remember (splitGenericValue gv (z - size_chunk m1)) as R.
-    destruct R as [[gvl' gvr']|]; inv H0.
-    apply chunk_matched_cons_inv in J.
-    destruct J as [gv2 [v3 [m3 [v4 [J1 [J2' J3']]]]]]; subst.
-    inv J1. inv J3'.
-    symmetry in HeqR.
-    eapply IHgv in HeqR; eauto.
-    destruct HeqR as [gvl'0 [gvr' [J4 [J5 [J6 [J7 J8]]]]]].
-    rewrite J4.     
-    exists ((v4, m3) :: gvl'0). exists gvr'. 
-    split; auto using gv_inject_cons_intro, chunk_matched_cons_intro.
-Qed.
-   
-Lemma simulation__splitGenericValue_none : forall mi gv gv' z,
-  chunk_matched gv gv' ->
-  gv_inject mi gv gv' ->
-  splitGenericValue gv z = None ->
-  splitGenericValue gv' z = None.
-Proof.
-  induction gv; simpl; intros gv' z J H H0.
-    apply gv_inject_nil_inv in H. subst.
-    simpl.
-    destruct (zeq z 0); inv H0. 
-    destruct (zlt z 0); inv H1; auto.
-
-    apply gv_inject_cons_inv in H. 
-    destruct H as [gv2' [v1 [m1 [v2 [m2 [J1 [J2 [J3 J4]]]]]]]]; subst.
-    simpl.
-    destruct (zeq z 0); inv H0. 
-    destruct (zlt z 0); inv H1; auto.
-    remember (splitGenericValue gv (z - size_chunk m1)) as R.
-    destruct R as [[gvl' gvr']|]; inv H0.
-    apply chunk_matched_cons_inv in J.
-    destruct J as [gv2 [v3 [m3 [v4 [J1 [J2' J3']]]]]]; subst.
-    inv J1. inv J3'.
-    symmetry in HeqR.
-    eapply IHgv in HeqR; eauto.
-    rewrite HeqR; auto.
-Qed.
-
-Lemma simulation__extractGenericValue : forall mi gv1 gv1' TD t1 l0 gv,
-  chunk_matched gv1 gv1' ->
-  gv_inject mi gv1 gv1' ->
-  extractGenericValue TD t1 gv1 l0 = Some gv ->
-  exists gv',
-    extractGenericValue TD t1 gv1' l0 = Some gv' /\
-    gv_inject mi gv gv'.
-Proof.
-  intros mi gv1 gv1' TD t1 l0 gv J H H0.
-  unfold extractGenericValue in *.
-  destruct (intConsts2Nats TD l0); inv H0; 
-    try solve [exists gundef; auto using gv_inject_gundef].
-  destruct (mgetoffset TD t1 l1); inv H2;
-    try solve [exists gundef; auto using gv_inject_gundef].
-  unfold mget in *. 
-  destruct (getTypeStoreSize TD t1); inv H1; 
-    try solve [exists gundef; auto using gv_inject_gundef].
-  remember (splitGenericValue gv1 (Int.signed 31 i0)) as R.
-  destruct R as [[gvl gvr]|].
-    symmetry in HeqR.
-    eapply simulation__splitGenericValue_some in HeqR; eauto.      
-    destruct HeqR as [gvl' [gvr' [J1 [J2 [J3 [J4 J5]]]]]].
-    simpl. rewrite J1.
-    remember (splitGenericValue gvr (Z_of_nat n)) as R1.
-    destruct R1 as [[gvrl gvrr]|]; inv H2.
-      symmetry in HeqR1.
-      eapply simulation__splitGenericValue_some in HeqR1; eauto.      
-      destruct HeqR1 as [gvrl' [gvrr' [J1' [J2' [J3' [J4' J5']]]]]].
-      simpl. rewrite J1'. eauto.
-
-      symmetry in HeqR1.
-      eapply simulation__splitGenericValue_none in HeqR1; eauto.      
-      rewrite HeqR1.     
-      exists gundef. auto using gv_inject_gundef.
-    symmetry in HeqR.
-    eapply simulation__splitGenericValue_none in HeqR; eauto.      
-    rewrite HeqR. inv H2.    
-    exists gundef. auto using gv_inject_gundef.
-Qed.
-
-
-Lemma gv_inject_length_eq : forall mi gv1 gv2,
-  gv_inject mi gv1 gv2 -> length gv1 = length gv2.
-Proof.
-  induction gv1; intros.
-    apply gv_inject_nil_inv in H. subst.
-    simpl. auto.
-
-    apply gv_inject_cons_inv in H. 
-    destruct H as [gv2' [v1 [m1 [v2 [m2 [J1 [J2 [J3 J4]]]]]]]]; subst.
-    simpl. eauto.
-Qed.
-
-Lemma simulation__insertGenericValue: forall mi gv1 gv1' TD t1 l0 gv t2 gv2 gv2',
-  chunk_matched gv1 gv1' ->
-  chunk_matched gv2 gv2' ->
-  gv_inject mi gv1 gv1' ->
-  gv_inject mi gv2 gv2' ->
-  insertGenericValue TD t1 gv1 l0 t2 gv2 = Some gv ->
-  exists gv',
-    insertGenericValue TD t1 gv1' l0 t2 gv2' = Some gv' /\
-    gv_inject mi gv gv'.
-Proof.
-  intros mi gv1 gv1' TD t1 l0 gv t2 gv2 gv2' JJ JJ' H H0 H1.
-  unfold insertGenericValue in *.
-  destruct (intConsts2Nats TD l0); inv H1; 
-    try solve [exists gundef; auto using gv_inject_gundef].
-  destruct (mgetoffset TD t1 l1); inv H3;
-    try solve [exists gundef; auto using gv_inject_gundef].
-  unfold mset in *. 
-  destruct (getTypeStoreSize TD t2); inv H2; 
-    try solve [exists gundef; auto using gv_inject_gundef].
-  assert (J:=@gv_inject_length_eq mi gv2 gv2' H0). 
-  rewrite <- J. simpl.
-  destruct (n =n= length gv2); subst;
-    try solve [inv H3; exists gundef; auto using gv_inject_gundef].
-  remember (splitGenericValue gv1 (Int.signed 31 i0)) as R.
-  destruct R as [[gvl gvr]|].
-    symmetry in HeqR.
-    eapply simulation__splitGenericValue_some in HeqR; eauto.      
-    destruct HeqR as [gvl' [gvr' [J1 [J2 [J3 [J4 J5]]]]]].
-    simpl. rewrite J1.
-    remember (splitGenericValue gvr (Z_of_nat n)) as R1.
-    destruct R1 as [[gvrl gvrr]|]; inv H3.
-      symmetry in HeqR1.
-      eapply simulation__splitGenericValue_some in HeqR1; eauto.      
-      destruct HeqR1 as [gvrl' [gvrr' [J1' [J2' [J3' [J4' J5']]]]]].
-      simpl. rewrite J1'. 
-      exists (gvl' ++ gv2' ++ gvrr').
-      split; auto.
-        apply gv_inject_app; auto.
-        apply gv_inject_app; auto.
-
-      symmetry in HeqR1.
-      eapply simulation__splitGenericValue_none in HeqR1; eauto.      
-      rewrite HeqR1.     
-      exists gundef. auto using gv_inject_gundef.
-    symmetry in HeqR.
-    eapply simulation__splitGenericValue_none in HeqR; eauto.      
-    rewrite HeqR. inv H3.    
-    exists gundef. auto using gv_inject_gundef.
-Qed.
-
-Lemma simulation__eq__GV2int : forall mi gn gn' TD sz,
-  defined_gv gn ->
-  gv_inject mi gn gn' ->
-  GV2int TD sz gn = GV2int TD sz gn'.
-Proof.
-  intros mi gn gn' TD sz Hdef Hinj.
-  unfold GV2int.
-  destruct gn.
-    apply gv_inject_nil_inv in Hinj. subst. auto.
-
-    apply gv_inject_cons_inv in Hinj.
-    destruct Hinj as [gv2 [v1 [m1 [v2 [m2 [J1 [J2 [J3 J4]]]]]]]]; subst.
-    inv J3; auto.
-      destruct gn.   
-        apply gv_inject_nil_inv in J2. subst. auto.
-        apply gv_inject_cons_inv in J2.
-        destruct J2 as [gv2' [v1' [m1' [v2' [m2' [J1' [J2' [J3' J4']]]]]]]]; 
-          subst; auto.
-        destruct v2; auto.
-          destruct gv2; auto.
-          simpl in Hdef. contradict Hdef; auto.
-Qed.
-
-Lemma simulation__isGVZero : forall mi c c' TD,
-  defined_gv c ->
-  gv_inject mi c c' ->
-  isGVZero TD c = isGVZero TD c'.
-Proof.
-  intros mi c c' TD Hdef Hinj.
-  unfold isGVZero.   
-  erewrite simulation__eq__GV2int; eauto.
-Qed.
-
-Lemma simulation__mtrunc_refl : forall mi TD top t1 gv1 t2 gv2,
-  gv_inject mi gv1 gv1 ->
-  mtrunc TD top t1 gv1 t2 = Some gv2 ->
-  gv_inject mi gv2 gv2.
-Proof.
-  intros.
-  apply gv_inject__val_inject with (TD:=TD) in H.
-  destruct H as [v1 [v2 [J1 [J2 J3]]]].
-  unfold mtrunc in *.
-  rewrite J1 in H0. unfold gv_inject.
-  rewrite J1 in J2. inv J2.
-  destruct v2; try (inv J3); try solve [inv H0; simpl; auto].
-    destruct t1; try solve [
-      inv H0; simpl; auto |
-      destruct t2; try solve 
-        [inv H0; simpl; auto | inv H0; simpl; destruct (le_lt_dec wz s0); auto]
-    ].
-
-    destruct t1; try solve [
-      inv H0; simpl; auto |
-      destruct t2; try solve [
-        inv H0; simpl; auto |
-        destruct (floating_point_order f1 f0); try solve [
-          destruct f1; try solve [inv H0; simpl; auto] |
-          inv H0; simpl; auto
-        ]
-      ]
-    ].
-Qed.
-
-Lemma simulation__mext_refl : forall mi TD eop t1 gv1 t2 gv2,
-  gv_inject mi gv1 gv1 ->
-  mext TD eop t1 gv1 t2 = Some gv2 ->
-  gv_inject mi gv2 gv2.
-Proof.
-  intros. assert (J0:=H).
-  apply gv_inject__val_inject with (TD:=TD) in H.
-  destruct H as [v1 [v2 [J1 [J2 J3]]]].
-  unfold mext in *.
-  rewrite J1 in H0. unfold gv_inject.
-  rewrite J1 in J2. inv J2.
-  destruct t1; destruct t2; inv H0; simpl; auto.
-    destruct v2; inv H1; simpl; auto.
-    destruct eop; inv H0; simpl; auto.
-    destruct (floating_point_order f f0); inv H1; simpl; auto.
-    destruct v2; inv H0; simpl; auto.
-    destruct eop; inv H1; simpl; auto.
-Qed.
-
-Lemma simulation__mbop_refl : forall mi TD op bsz gv1 gv2 gv3,
-  gv_inject mi gv1 gv1 ->
-  gv_inject mi gv2 gv2 ->
-  mbop TD op bsz gv1 gv2 = Some gv3 ->
-  gv_inject mi gv3 gv3.
-Proof.
-  intros. assert (J0:=H0). assert (J:=H).
-  apply gv_inject__val_inject with (TD:=TD) in H.
-  destruct H as [v1 [v1' [J1 [J2 J3]]]].
-  apply gv_inject__val_inject with (TD:=TD) in H0.
-  destruct H0 as [v2 [v2' [J1' [J2' J3']]]].
-  rewrite J1 in J2. inv J2.
-  rewrite J1' in J2'. inv J2'.
-  unfold mbop in *.
-  rewrite J1 in H1. rewrite J1' in H1. 
-  destruct v1';
-    try solve [inv H1; auto using gv_inject_gundef].
-  destruct v2';
-    try solve [inv H1; auto using gv_inject_gundef].
-  destruct (eq_nat_dec (wz + 1) (Size.to_nat bsz)); 
-     try solve [inv H1; auto using gv_inject_gundef].
-  destruct op; inv H1; try (apply gv_inject_nptr_val_refl; auto).
-       apply add_isnt_ptr.
-       apply sub_isnt_ptr.
-       apply mul_isnt_ptr.
-       apply divu_isnt_ptr.
-       apply divs_isnt_ptr.
-       apply modu_isnt_ptr.
-       apply mods_isnt_ptr.
-       apply shl_isnt_ptr.
-       apply shrx_isnt_ptr.
-       apply shr_isnt_ptr.
-       apply and_isnt_ptr.
-       apply or_isnt_ptr.
-       apply xor_isnt_ptr.
-Qed.
-
-Lemma simulation__mfbop_refl : forall mi TD op fp gv1 gv2 gv3,
-  gv_inject mi gv1 gv1 ->
-  gv_inject mi gv2 gv2 ->
-  mfbop TD op fp gv1 gv2 = Some gv3 ->
-  gv_inject mi gv3 gv3.
-Proof.
-  intros. assert (J0:=H0). assert (J:=H).
-  apply gv_inject__val_inject with (TD:=TD) in H.
-  destruct H as [v1 [v1' [J1 [J2 J3]]]].
-  apply gv_inject__val_inject with (TD:=TD) in H0.
-  destruct H0 as [v2 [v2' [J1' [J2' J3']]]].
-  rewrite J1 in J2. inv J2.
-  rewrite J1' in J2'. inv J2'.
-  unfold mfbop in *.
-  rewrite J1 in H1. rewrite J1' in H1. 
-  destruct v1';
-    try solve [inv H1; auto using gv_inject_gundef].
-  destruct v2';
-    try solve [inv H1; auto using gv_inject_gundef].
-  destruct fp; try solve [inv H1; auto using gv_inject_gundef].
-  destruct op; inv H1; 
-    try (apply gv_inject_nptr_val_refl; try solve [auto | intro; congruence]).
-  destruct op; inv H1; 
-    try (apply gv_inject_nptr_val_refl; try solve [auto | intro; congruence]).
-Qed.
-
-Lemma simulation__mcast_refl : forall mi TD op t1 t2 gv1 gv2,
-  gv_inject mi gv1 gv1 ->
-  mcast TD op t1 gv1 t2 = Some gv2 ->
-  gv_inject mi gv2 gv2.
-Proof.
-  intros.  assert (J:=H).
-  apply gv_inject__val_inject with (TD:=TD) in H.
-  destruct H as [v1 [v1' [J1 [J2 J3]]]].
-  rewrite J1 in J2. inv J2.
-  unfold mcast, mbitcast in *.
-  destruct op; 
-    try solve [
-      inv H0; auto using gv_inject_gundef |
-      destruct t1; destruct t2; inv H0; auto using gv_inject_gundef
-    ].
-Qed.
-
-Lemma simulation__micmp_refl : forall mi TD c t gv1 gv2 gv3,
-  gv_inject mi gv1 gv1 ->
-  gv_inject mi gv2 gv2 ->
-  micmp TD c t gv1 gv2 = Some gv3 ->
-  gv_inject mi gv3 gv3.
-Proof.
-  intros. assert (J0:=H0). assert (J:=H).
-  apply gv_inject__val_inject with (TD:=TD) in H.
-  destruct H as [v1 [v1' [J1 [J2 J3]]]].
-  apply gv_inject__val_inject with (TD:=TD) in H0.
-  destruct H0 as [v2 [v2' [J1' [J2' J3']]]].
-  rewrite J1 in J2. inv J2.
-  rewrite J1' in J2'. inv J2'.
-  unfold micmp, micmp_int in *.
-  rewrite J1 in H1. rewrite J1' in H1. 
-  destruct t; try solve [inv H1; auto using gv_inject_gundef].
-  destruct v1'; try solve [inv H1; auto using gv_inject_gundef].
-  destruct v2'; try solve [inv H1; auto using gv_inject_gundef].
-  destruct c; inv H1; 
-        try (apply gv_inject_nptr_val_refl; try solve 
-            [auto | apply cmp_isnt_ptr | apply cmpu_isnt_ptr]).
-Qed.
-
-Lemma simulation__mfcmp_refl : forall mi TD c t gv1 gv2 gv3,
-  gv_inject mi gv1 gv1 ->
-  gv_inject mi gv2 gv2 ->
-  mfcmp TD c t gv1 gv2 = Some gv3 ->
-  gv_inject mi gv3 gv3.
-Proof.
-  intros. assert (J0:=H0). assert (J:=H).
-  apply gv_inject__val_inject with (TD:=TD) in H.
-  destruct H as [v1 [v1' [J1 [J2 J3]]]].
-  apply gv_inject__val_inject with (TD:=TD) in H0.
-  destruct H0 as [v2 [v2' [J1' [J2' J3']]]].
-  rewrite J1 in J2. inv J2.
-  rewrite J1' in J2'. inv J2'.
-  unfold mfcmp in *.
-  rewrite J1 in H1. rewrite J1' in H1. 
-  destruct v1'; try solve [inv H1; auto using gv_inject_gundef].
-  destruct v2'; try solve [inv H1; auto using gv_inject_gundef].
-  destruct t; try solve [inv H1; auto using gv_inject_gundef].
-  destruct c; inv H1; try (
-    apply gv_inject_nptr_val_refl; try solve 
-            [auto | apply val_of_bool_isnt_ptr | apply Vfalse_isnt_ptr | 
-             apply Vtrue_isnt_ptr]
-    ).
-    auto using gv_inject_gundef.
-    auto using gv_inject_gundef.
-  destruct c; inv H1; try (
-    apply gv_inject_nptr_val_refl; try solve 
-            [auto | apply val_of_bool_isnt_ptr | apply Vfalse_isnt_ptr | 
-             apply Vtrue_isnt_ptr]
-    ).
-    auto using gv_inject_gundef.
-    auto using gv_inject_gundef.
-Qed.
-
-Lemma simulation__mgep_refl : forall mi TD v v0 t0 l1,
-  Values.val_inject mi v v ->
-  mgep TD t0 v l1 = Some v0 ->
-  Values.val_inject mi v0 v0.
-Proof.
-  intros.
-  unfold mgep in *.
-  destruct v; tinv H0.
-  destruct l1; tinv H0.
-  destruct (mgetoffset TD (typ_array 0%nat t0) (z :: l1)); tinv H0.
-  inv H0.
-  inversion H. subst i0 b ofs1 b1.
-  eapply val_inject_ptr; eauto.
-    assert (Int.add 31 ofs2 (Int.repr 31 delta) = 
-            Int.add 31 (Int.repr 31 delta) ofs2) as EQ.
-      rewrite <- Int.add_commut. auto. 
-    symmetry.
-    rewrite Int.add_commut. 
-    rewrite <- Int.add_assoc.
-    rewrite <- EQ.   
-    rewrite <- H5.
-    auto.
-Qed.
-
-
-Lemma GV2ptr_refl : forall mi TD gv v,
-  gv_inject mi gv gv ->
-  GV2ptr TD (getPointerSize TD) gv = Some v ->
-  val_inject mi v v.
-Proof.
-  intros.
-  unfold GV2ptr in H0.
-  destruct gv; tinv H0.
-  destruct p; tinv H0.
-  destruct v0; tinv H0.
-  destruct gv; tinv H0.
-  inv H0.
-  unfold gv_inject in H.
-  simpl in H. inv H; auto.
-Qed.
-
-
-Lemma simulation__splitGenericValue_refl : forall mi gv z gvl gvr,
-  gv_inject mi gv gv ->
-  splitGenericValue gv z = Some (gvl, gvr) ->
-  gv_inject mi gvl gvl /\
-  gv_inject mi gvr gvr.
-Proof.
-  induction gv; simpl; intros.
-    apply gv_inject_nil_inv in H. subst.
-    simpl.
-    destruct (zeq z 0); inv H0. 
-      auto using gv_inject_nil_refl.
-      destruct (zlt z 0); inv H2.
-
-    apply gv_inject_cons_inv in H. 
-    destruct H as [gv2' [v1 [m1 [v2 [m2 [J1 [J2 [J3 J4]]]]]]]]; subst.
-    simpl.
-    destruct (zeq z 0); inv H0. 
-      inv J1.
-      split; auto using gv_inject_nil_refl, gv_inject_cons_intro.
-    destruct (zlt z 0); inv H1.
-    remember (splitGenericValue gv (z - size_chunk m1)) as R.
-    destruct R as [[gvl' gvr']|]; inv H0.
-    symmetry in HeqR. inv J1.
-    eapply IHgv in HeqR; eauto.
-    destruct HeqR as [J5 J6].
-    split; auto using gv_inject_cons_intro.
-Qed.
-
-Lemma simulation__extractGenericValue_refl : forall mi gv1 TD t1 l0 gv,
-  gv_inject mi gv1 gv1 ->
-  extractGenericValue TD t1 gv1 l0 = Some gv ->
-  gv_inject mi gv gv.
-Proof.
-  intros.
-  unfold extractGenericValue in *.
-  destruct (intConsts2Nats TD l0); inv H0;
-    try solve [auto using gv_inject_gundef].
-  destruct (mgetoffset TD t1 l1); inv H2;
-    try solve [auto using gv_inject_gundef].
-  unfold mget in *. 
-  destruct (getTypeStoreSize TD t1); inv H1; 
-    try solve [auto using gv_inject_gundef].
-  remember (splitGenericValue gv1 (Int.signed 31 i0)) as R.
-  destruct R as [[gvl gvr]|]; inv H2;
-    try solve [auto using gv_inject_gundef].
-  symmetry in HeqR.
-  eapply simulation__splitGenericValue_refl in HeqR; eauto.      
-  destruct HeqR as [J2 J3].
-  remember (splitGenericValue gvr (Z_of_nat n)) as R1.
-  destruct R1 as [[gvrl gvrr]|]; inv H1;
-    try solve [auto using gv_inject_gundef].
-  symmetry in HeqR1.
-  eapply simulation__splitGenericValue_refl in HeqR1; eauto.      
-  destruct HeqR1; auto.
-Qed.
-
-Lemma simulation__insertGenericValue_refl : forall mi gv1 TD t1 l0 gv t2 gv2,
-  gv_inject mi gv1 gv1 ->
-  gv_inject mi gv2 gv2 ->
-  insertGenericValue TD t1 gv1 l0 t2 gv2 = Some gv ->
-  gv_inject mi gv gv.
-Proof.
-  intros.
-  unfold insertGenericValue in *.
-  destruct (intConsts2Nats TD l0); inv H1; 
-    try solve [auto using gv_inject_gundef].
-  destruct (mgetoffset TD t1 l1); inv H3;
-    try solve [auto using gv_inject_gundef].
-  unfold mset in *. 
-  destruct (getTypeStoreSize TD t2); inv H2; 
-    try solve [ auto using gv_inject_gundef].
-  destruct (n =n= length gv2); subst;
-    try solve [inv H3; auto using gv_inject_gundef].
-  remember (splitGenericValue gv1 (Int.signed 31 i0)) as R.
-  destruct R as [[gvl gvr]|]; inv H3;
-    try solve [auto using gv_inject_gundef].
-  symmetry in HeqR.
-  eapply simulation__splitGenericValue_refl in HeqR; eauto.      
-  destruct HeqR as [J2 J3].
-  remember (splitGenericValue gvr (Z_of_nat n)) as R1.
-  destruct R1 as [[gvrl gvrr]|]; inv H2;
-    try solve [auto using gv_inject_gundef].
-  symmetry in HeqR1.
-  eapply simulation__splitGenericValue_refl in HeqR1; eauto.      
-  destruct HeqR1.
-  apply gv_inject_app; auto.
-  apply gv_inject_app; auto.
-Qed.
-
-Definition sb_mem_inj__const2GV_prop (c:const) := forall maxb mi Mem1 Mem2 TD gl 
-    gv t,
-  wf_sb_mi maxb mi Mem1 Mem2 ->
-  wf_globals maxb gl -> 
-  _const2GV TD gl c = Some (gv,t) ->
-  gv_inject mi gv gv.
-
-Definition sb_mem_inj__list_const2GV_prop (lc:list_const) := 
-  forall maxb mi Mem1 Mem2 TD gl,
-  wf_sb_mi maxb mi Mem1 Mem2 ->
-  wf_globals maxb gl -> 
-  (forall gv, 
-    _list_const_arr2GV TD gl lc = Some gv ->
-    gv_inject mi gv gv
-  ) /\
-  (forall gv t a, 
-    _list_const_struct2GV TD gl lc = Some (gv,t,a) ->
-    gv_inject mi gv gv
-  ).
-
-Lemma sb_mem_inj__const2GV_mutrec :
-  (forall c, sb_mem_inj__const2GV_prop c) *
-  (forall lc, sb_mem_inj__list_const2GV_prop lc).
-Proof.
-  apply const_mutrec; 
-    unfold sb_mem_inj__const2GV_prop, sb_mem_inj__list_const2GV_prop;
-    intros; simpl in *; eauto.
-Case "zero".
-  remember (zeroconst2GV TD t) as R.
-  destruct R; inv H1.
-  eauto using zeroconst2GV__gv_inject_refl.
-Case "int".
-  inv H1.
-  unfold val2GV, gv_inject; simpl; auto.
-Case "float".
-  destruct f; inv H1; unfold val2GV, gv_inject; simpl; auto.
-Case "undef".
-  remember (getTypeSizeInBits TD t) as R.
-  destruct R; inv H1; unfold val2GV, gv_inject; simpl; auto.
-Case "null".
-  inv H1. unfold val2GV, gv_inject; simpl; auto.
-      apply val_cons_inject; auto.
-      apply val_inject_ptr with (delta:=0); auto.
-      destruct H. auto.
-Case "arr". 
-  eapply H with (TD:=TD)(gl:=gl) in H1; eauto.
-  destruct H1; eauto.
-  remember (_list_const_arr2GV TD gl l0) as R.
-  destruct R; inv H2. eauto.
-Case "struct". 
-  eapply H with (TD:=TD)(gl:=gl) in H1; eauto.
-  destruct H1 as [H00 H01].
-  remember (_list_const_struct2GV TD gl l0) as R.
-  destruct R as [[[gv1 t1] a1]|]; inv H2.
-  destruct (getTypeAllocSize TD (typ_struct t1)); try solve [inv H3].
-  destruct l0; inv H3.
-    apply gv_inject_uninits.
-    apply gv_inject_app; eauto.
-      apply gv_inject_uninits.
-Case "gid".
-  remember (lookupAL GenericValue gl i0) as R.
-  destruct R; inv H1.
-  eauto using global_gv_inject_refl.
-Case "trunc".
-  remember (_const2GV TD gl c) as R.
-  destruct R as [[gv1 t1']|]; try solve [inv H2].
-  symmetry in HeqR.
-  eapply H in HeqR; eauto.
-  remember (mtrunc TD t t1' gv1 t0) as R1.
-  destruct R1; inv H2.
-  symmetry in HeqR1.
-  eapply simulation__mtrunc_refl in HeqR1; eauto.
-Case "ext".
-  remember (_const2GV TD gl c) as R.
-  destruct R as [[gv1 t1']|]; tinv H2.
-  symmetry in HeqR.
-  eapply H in HeqR; eauto.
-  remember (mext TD e t1' gv1 t) as R1.
-  destruct R1; inv H2.
-  symmetry in HeqR1.
-  eapply simulation__mext_refl in HeqR1; eauto.
-Case "cast".
-  remember (_const2GV TD gl c0) as R.
-  destruct R as [[gv1 t1']|]; tinv H2.
-  symmetry in HeqR.
-  eapply H in HeqR; eauto.
-  remember (mcast TD c t1' gv1 t) as R1.
-  destruct R1; inv H2.
-  symmetry in HeqR1.
-  eapply simulation__mcast_refl in HeqR1; eauto.
-Case "gep".
-  remember (_const2GV TD gl c) as R1.
-  destruct R1 as [[gv1 t1]|]; tinv H3.
-  destruct t1; tinv H3.
-  remember (getConstGEPTyp l0 (typ_pointer t1)) as R2.
-  destruct R2; tinv H3.
-  remember (GV2ptr TD (getPointerSize TD) gv1) as R3.
-  destruct R3; tinv H3.
-    remember (intConsts2Nats TD l0) as R4.
-    destruct R4; tinv H3.
-      remember (mgep TD t1 v l1) as R5.
-      destruct R5; inv H3.
-        symmetry in HeqR1.
-        eapply H in HeqR1; eauto.
-        symmetry in HeqR5.
-        eapply simulation__mgep_refl with (mi:=mi) in HeqR5; 
-          eauto using GV2ptr_refl.
-        unfold ptr2GV, val2GV, gv_inject. simpl. auto.
-
-        apply gv_inject_gundef.
-      inv H3. apply gv_inject_gundef.
-    inv H3. apply gv_inject_gundef.
-Case "select".
-  remember (_const2GV TD gl c) as R3.
-  destruct R3 as [[gv3 t3]|]; tinv H4.
-  remember (_const2GV TD gl c0) as R4.
-  destruct R4 as [[gv4 t4]|]; tinv H4.
-  remember (_const2GV TD gl c2) as R5.
-  destruct R5; tinv H4.
-  destruct (isGVZero TD gv3); inv H4; eauto.
-Case "icmp".
-  remember (_const2GV TD gl c0) as R3.
-  destruct R3 as [[gv3 t3]|]; tinv H3.
-  remember (_const2GV TD gl c2) as R4.
-  destruct R4 as [[gv4 t4]|]; tinv H3.
-  symmetry in HeqR3. 
-  eapply H in HeqR3; eauto.
-  symmetry in HeqR4. 
-  eapply H0 in HeqR4; eauto.
-  remember (micmp TD c t3 gv3 gv4) as R1.
-  destruct R1; inv H3.
-  symmetry in HeqR1.
-  eapply simulation__micmp_refl in HeqR1; eauto.
-Case "fcmp".
-  remember (_const2GV TD gl c) as R3.
-  destruct R3 as [[gv3 t3]|]; tinv H3.
-  destruct t3; tinv H3.  
-  remember (_const2GV TD gl c0) as R4.
-  destruct R4 as [[gv4 t4]|]; tinv H3.
-  symmetry in HeqR3. 
-  eapply H in HeqR3; eauto.
-  symmetry in HeqR4. 
-  eapply H0 in HeqR4; eauto.
-  remember (mfcmp TD f f0 gv3 gv4) as R1.
-  destruct R1; inv H3.
-  symmetry in HeqR1.
-  eapply simulation__mfcmp_refl in HeqR1; eauto.
-Case "extractValue". 
-  remember (_const2GV TD gl c) as R.
-  destruct R as [[gv1 t1]|]; tinv H3.
-  remember (getSubTypFromConstIdxs l0 t1) as R2.
-  destruct R2; tinv H3.   
-  remember (extractGenericValue TD t1 gv1 l0) as R3.
-  destruct R3; inv H3.   
-  symmetry in HeqR3.
-  eapply simulation__extractGenericValue_refl in HeqR3; eauto.
-Case "insertValue". 
-  remember (_const2GV TD gl c) as R.
-  destruct R as [[gv1 t1]|]; tinv H4.
-  remember (_const2GV TD gl c0) as R2.
-  destruct R2 as [[gv2 t2]|]; tinv H4.
-  remember (insertGenericValue TD t1 gv1 l0 t2 gv2) as R3.
-  destruct R3; inv H4.   
-  symmetry in HeqR3.
-  eapply simulation__insertGenericValue_refl in HeqR3; eauto.
-Case "bop".
-  remember (_const2GV TD gl c) as R3.
-  destruct R3 as [[gv3 t3]|]; tinv H3.
-  destruct t3; tinv H3.
-  remember (_const2GV TD gl c0) as R4.
-  destruct R4 as [[gv4 t4]|]; tinv H3.
-  remember (mbop TD b s gv3 gv4) as R1.
-  destruct R1; inv H3.
-  symmetry in HeqR1.
-  eapply simulation__mbop_refl in HeqR1; eauto.
-Case "fbop".
-  remember (_const2GV TD gl c) as R3.
-  destruct R3 as [[gv3 t3]|]; tinv H3.
-  destruct t3; tinv H3.
-  remember (_const2GV TD gl c0) as R4.
-  destruct R4 as [[gv4 t4]|]; tinv H3.
-  remember (mfbop TD f f0 gv3 gv4) as R1.
-  destruct R1; inv H3.
-  symmetry in HeqR1.
-  eapply simulation__mfbop_refl in HeqR1; eauto.
-Case "nil".
-  split.
-    intros gv J.
-    inv J. apply gv_inject_nil_refl; auto.
-    intros gv t a J.
-    inv J. apply gv_inject_nil_refl; auto.
-Case "cons".
-  split; intros.
-    remember (_list_const_arr2GV TD gl l0) as R3.
-    destruct R3 as [gv3|]; tinv H3.
-    remember (_const2GV TD gl c) as R4.
-    destruct R4 as [[gv4 t4]|]; tinv H3.
-    symmetry in HeqR4.
-    eapply H in HeqR4; eauto.
-    eapply H0 with (TD:=TD) in H1; eauto.
-    destruct H1 as [J3 J4]; auto.
-    destruct (getTypeStoreSize TD t4); tinv H3.
-    destruct (getTypeAllocSize TD t4); inv H3.
-      apply gv_inject_app.
-        apply gv_inject_app; auto.
-        apply gv_inject_uninits.
-
-    remember (_list_const_struct2GV TD gl l0) as R3.
-    destruct R3 as [[[gv3 t3] a3]|]; tinv H3.
-    remember (_const2GV TD gl c) as R4.
-    destruct R4 as [[gv4 t4]|]; tinv H3.
-    symmetry in HeqR4.
-    eapply H in HeqR4; eauto.
-    eapply H0 with (TD:=TD) in H1; eauto.
-    destruct H1 as [J3 J4]; auto.
-    destruct (getTypeStoreSize TD t4); tinv H3.
-    destruct (getTypeAllocSize TD t4); inv H3.
-      apply gv_inject_app; eauto.
-        apply gv_inject_app; auto.
-        apply gv_inject_uninits.
-Qed.
-
-Lemma sb_mem_inj__const2GV : forall maxb mi Mem Mem' TD gl c gv,
-  wf_sb_mi maxb mi Mem Mem' ->
-  wf_globals maxb gl -> 
-  const2GV TD gl c = Some gv ->
-  gv_inject mi gv gv.
-Proof.
-  destruct sb_mem_inj__const2GV_mutrec as [J _].
-  unfold sb_mem_inj__const2GV_prop in J. 
-  intros.
-  unfold const2GV in H1.
-  remember (_const2GV TD gl c) as R.
-  destruct R as [[? ?]|]; inv H1; eauto.
 Qed.
 
 Lemma simulation__getOperandValue : forall maxb mi rm rm2 lc lc2 TD Mem Mem2 
@@ -1971,25 +145,6 @@ Proof.
   eapply simulation__mfbop in H3; eauto.
 Qed.
 
-Fixpoint gvs_inject mi gvs1 gvs2 : Prop :=
-match (gvs1, gvs2) with
-| (nil, nil) => True
-| (gv1::gvs1', gv2::gvs2') => gv_inject mi gv1 gv2 /\ gvs_inject mi gvs1' gvs2'
-| _ => False
-end.
-
-Lemma simulation__GVs2Nats : forall mi TD vidxs vidxs',
-  defined_gvs vidxs ->
-  gvs_inject mi vidxs vidxs' ->
-  GVs2Nats TD vidxs = GVs2Nats TD vidxs'.
-Proof.
-  induction vidxs; intros vidxs' Hdefs Hinj.
-    destruct vidxs'; inv Hinj; simpl; auto.
-    destruct vidxs'; simpl in *; inv Hinj; auto.
-      destruct Hdefs as [J1 J2].
-      erewrite simulation__eq__GV2int; eauto.      
-      erewrite IHvidxs; eauto.
-Qed.
 
 Lemma simulation__GEP : forall maxb mi TD Mem Mem2 inbounds0 vidxs vidxs' gvp1 
     gvp gvp' t,
@@ -2201,7 +356,7 @@ Proof.
 
     destruct a. simpl in *.
     destruct H as [J1 J2].
-    destruct (i0 == i1); subst; eauto.
+    destruct (i0 == i2); subst; eauto.
       inv H2.
       unfold GV2val in H1.
       destruct g0; inv H1.
@@ -2226,28 +381,6 @@ Proof.
   exists ex_ids3. exists cs1. exists cs2. eauto.
 Qed.
 
-
-Lemma gv_inject_ptr_inv : forall mi b ofs gv' cm,
-  gv_inject mi ((Vptr b ofs,cm)::nil) gv' ->
-  exists b', exists ofs', exists cm,
-    gv' = (Vptr b' ofs', cm)::nil /\
-    val_inject mi (Vptr b ofs) (Vptr b' ofs').
-Proof.
-  intros mi b ofs gv' cm J .
-  unfold gv_inject in J.
-  simpl in J.
-  destruct gv'; simpl in J.
-    inv J.
-
-    destruct p; simpl in J. 
-    destruct gv'; simpl in J.    
-      inv J. 
-      inv H2. exists b2. exists (Int.add 31 ofs (Int.repr 31 delta)). exists m.
-      split; eauto.
-
-      destruct p. destruct (split gv'). 
-      inv J. inv H4.
-Qed.
 
 Lemma mem_simulation__malloc : forall mi TD MM Mem Mem2 tsz gn align0 Mem' mb 
     mgb,
@@ -2546,32 +679,450 @@ Ltac invert_prop_reg_metadata :=
       inv H; subst; eauto
   end.
 
-Lemma reg_simulation__updateAddAL_md : forall mi TD gl f1 rm1 rm2 lc1 lc2 id0 
-    bgv1 bgv2 egv1 egv2 bid eid c ex_ids3 mgb M1 M2
+Lemma reg_simulation_spec : forall mi nts los gl f1 rm1 rm2 lc1 lc2 gv1 i0,
+  reg_simulation mi (los,nts) gl f1 rm1 rm2 lc1 lc2 ->
+  lookupAL GenericValue lc1 i0 = ret gv1 ->
+  i0 `in` (ids2atoms (getFdefLocs f1)).
+Proof.
+  intros.
+  destruct H as [_ [_ H]].
+  apply H in H0.
+  apply ids2atoms_dom; auto.
+Qed.
+
+Lemma in_singleton : forall a d, singleton a [<=] d <-> a `in` d.
+Proof.
+  intros.
+  unfold AtomSetImpl.Subset.
+  split; intros; eauto.
+    assert (a0 = a) as EQ. fsetdec.
+    subst. auto.
+Qed.      
+
+Lemma ids2atoms__in : forall a d, In a d <-> singleton a [<=] (ids2atoms d).
+Proof. 
+  induction d; simpl.
+    split; intros. 
+      inv H.
+
+      apply in_singleton in H. 
+      fsetdec.
+    destruct IHd as [J1 J2].
+    split; intros. 
+      destruct H as [H | H]; subst. 
+        fsetdec.        
+        apply J1 in H. fsetdec.
+        assert (a = a0 \/ a `in` (ids2atoms d)) as J.
+          fsetdec.
+        destruct J as [J | J]; subst; auto.
+          apply in_singleton in J. eauto.
+Qed.
+
+Lemma ids2atoms__notin : forall a d, ~ In a d <-> a `notin` (ids2atoms d).
+Proof. 
+  split; intros.  
+    destruct (AtomSetProperties.In_dec a (ids2atoms d)); auto.
+      apply in_singleton in i0.
+      apply ids2atoms__in in i0. congruence.
+    destruct (in_dec eq_atom_dec a d); auto.
+      apply ids2atoms__in in i0.
+      apply in_singleton in i0. congruence.
+Qed.
+
+Lemma incl_nil : forall A (d:list A), incl nil d.
+Proof. intros. intros x J. inv J. Qed.
+
+Lemma ids2atoms__inc : forall d1 d2,
+  incl d1 d2 <-> ids2atoms d1 [<=] ids2atoms d2.
+Proof.
+  intros.
+  split; intros.
+    induction d1; simpl.
+      fsetdec.
+      simpl_env in H.
+      assert (H':=H).
+      apply incl_app_invr in H.
+      apply incl_app_invl in H'.
+      apply IHd1 in H.      
+      assert (In a [a]) as Hin. simpl. auto.
+      apply H' in Hin.
+      apply ids2atoms__in in Hin.
+      fsetdec.
+    induction d1; simpl in *; auto using incl_nil.
+      intros x J.
+      simpl in J.
+      destruct J as [J | J]; subst.
+      apply ids2atoms__in. fsetdec.
+
+      revert J. revert x. 
+      apply IHd1. fsetdec.
+Qed.
+
+Lemma gen_metadata_id_spec : forall (ex_ids1 ex_ids0 : ids) i0 rm1
+  (Hin : i0 `in` ids2atoms ex_ids0)
+  (H1 : ids2atoms ex_ids0[<=]ids2atoms ex_ids1)
+  (H2 : AtomSetImpl.inter (ids2atoms ex_ids0) (codom rm1)[<=]empty)
+  (H3 : codom rm1[<=]ids2atoms ex_ids1)
+  (H4 : rm_codom_disjoint rm1)
+  (H6 : dom rm1[<=]ids2atoms ex_ids0)
+  (ex_ids5 : ids) (rm5 : rmap) 
+  (b : id) (e : id)
+  (Hgenid : gen_metadata_id ex_ids1 rm1 i0 = (b, e, ex_ids5, rm5)),
+   ids2atoms ex_ids1[<=]ids2atoms ex_ids5 /\
+   AtomSetImpl.inter (ids2atoms ex_ids0) (codom rm5)[<=]empty /\
+   codom rm5[<=]ids2atoms ex_ids5 /\
+   rm_codom_disjoint rm5 /\ dom rm5[<=]ids2atoms ex_ids0.
+Proof.
+  intros.
+      unfold gen_metadata_id in Hgenid.      
+      remember (atom_fresh_for_list ex_ids1) as R1.
+      destruct R1.
+      remember (atom_fresh_for_list (x::ex_ids1)) as R2.
+      destruct R2.
+      inv Hgenid.
+      assert (b `notin` ids2atoms ex_ids1) as Hnotinb.
+        apply ids2atoms__notin; auto.
+      assert (e `notin` ids2atoms (b::ex_ids1)) as Hnotine.
+        apply ids2atoms__notin; auto.
+      simpl in Hnotine.
+      destruct_notin.
+      simpl.
+      split. fsetdec.
+      split.
+        clear - H2 H1 NotInTac Hnotinb.
+        fsetdec.
+      split. clear - H3. fsetdec.
+      split.
+        clear HeqR1 HeqR2 n n0 Hnotine.
+        split. clear - Hin H1 Hnotinb. fsetdec.
+        split. clear - Hin H1 NotInTac. fsetdec.
+        split; auto.
+        split. clear - Hin H2. fsetdec.
+        split. clear - H3 H6 Hnotinb H1. fsetdec.
+        split; auto. 
+          clear - H3 H6 NotInTac H1. fsetdec.
+ 
+        simpl. clear - H6 Hin.
+        intros x J. 
+        assert (x = i0 \/ x `in` (dom rm1)) as H.
+          fsetdec.
+        destruct H as [H | H]; subst; auto.
+Qed.      
+  
+Lemma gen_metadata_args_spec : forall ex_ids0 la rm1 rm2 ex_ids1 ex_ids2, 
+  incl (getArgsIDs la) ex_ids0 ->
+  ids2atoms ex_ids0 [<=] ids2atoms ex_ids1 ->
+  AtomSetImpl.inter (ids2atoms ex_ids0) (codom rm1) [<=] {} ->
+  codom rm1 [<=] ids2atoms ex_ids1 ->
+  rm_codom_disjoint rm1 ->
+  dom rm1 [<=] ids2atoms ex_ids0 ->
+  gen_metadata_args ex_ids1 rm1 la = (ex_ids2,rm2) ->
+  ids2atoms ex_ids1 [<=] ids2atoms ex_ids2 /\
+  AtomSetImpl.inter (ids2atoms ex_ids0) (codom rm2) [<=] {} /\
+  codom rm2 [<=] ids2atoms ex_ids2 /\
+  rm_codom_disjoint rm2 /\
+  dom rm2 [<=] ids2atoms ex_ids0.
+Proof.
+  induction la; simpl; intros rm1 rm2 ex_ids1 ex_ids2 Hinc H1 H2 H3 H4 H6 H5.
+    inv H5. split; auto. fsetdec.
+
+    destruct a. destruct p.
+    assert (i0 `in` ids2atoms ex_ids0) as Hin.
+      apply ids2atoms__inc in Hinc.
+      simpl in Hinc. fsetdec.
+    simpl_env in Hinc. apply incl_app_invr in Hinc.
+    destruct (isPointerTypB t).
+      case_eq (gen_metadata_id ex_ids1 rm1 i0).
+      intros [[b e] ex_ids5] rm5 Hgenid.
+      rewrite Hgenid in H5.
+      eapply gen_metadata_id_spec in Hgenid; eauto.
+      destruct Hgenid as [J8 [J9 [J10 [J11 J12]]]].
+      assert (ids2atoms ex_ids0[<=]ids2atoms ex_ids5) as Hinc'.
+        clear - H1 J8. fsetdec.
+      apply IHla in H5; auto.
+      destruct H5 as [J1 [J2 [J3 J4]]].
+      split; auto. 
+         clear - J8 J1. fsetdec.
+
+      apply IHla in H5; auto.
+Qed.
+
+Lemma gen_metadata_phinodes_spec : forall ex_ids0 ps rm1 rm2 ex_ids1 ex_ids2,
+  incl (getPhiNodesIDs ps) ex_ids0 ->
+  ids2atoms ex_ids0 [<=] ids2atoms ex_ids1 ->
+  AtomSetImpl.inter (ids2atoms ex_ids0) (codom rm1) [<=] {} ->
+  codom rm1 [<=] ids2atoms ex_ids1 ->
+  rm_codom_disjoint rm1 ->
+  dom rm1 [<=] ids2atoms ex_ids0 ->
+  gen_metadata_phinodes ex_ids1 rm1 ps = (ex_ids2,rm2) ->
+  ids2atoms ex_ids1 [<=] ids2atoms ex_ids2 /\
+  AtomSetImpl.inter (ids2atoms ex_ids0) (codom rm2) [<=] {} /\
+  codom rm2 [<=] ids2atoms ex_ids2 /\
+  rm_codom_disjoint rm2 /\
+  dom rm2 [<=] ids2atoms ex_ids0.
+Proof.
+  induction ps; simpl; intros rm1 rm2 ex_ids1 ex_ids2 Hinc H1 H2 H3 H4 H6 H5.
+    inv H5. split; auto. fsetdec.
+
+    destruct a. simpl in *.
+    assert (i0 `in` ids2atoms ex_ids0) as Hin.
+      apply ids2atoms__inc in Hinc.
+      simpl in Hinc. fsetdec.
+    simpl_env in Hinc. apply incl_app_invr in Hinc.
+    destruct (isPointerTypB t).
+      case_eq (gen_metadata_id ex_ids1 rm1 i0).
+      intros [[b e] ex_ids5] rm5 Hgenid.
+      rewrite Hgenid in H5.
+      eapply gen_metadata_id_spec in Hgenid; eauto.
+      destruct Hgenid as [J8 [J9 [J10 [J11 J12]]]].
+      assert (ids2atoms ex_ids0[<=]ids2atoms ex_ids5) as Hinc'.
+        clear - H1 J8. fsetdec.
+      apply IHps in H5; auto.
+      destruct H5 as [J1 [J2 [J3 J4]]].
+      split; auto. 
+         clear - J8 J1. fsetdec.
+
+      apply IHps in H5; auto.
+Qed.
+
+Lemma gen_metadata_cmds_spec : forall nts ex_ids0 cs rm1 rm2 ex_ids1 ex_ids2, 
+  incl (getCmdsLocs cs) ex_ids0 ->
+  ids2atoms ex_ids0 [<=] ids2atoms ex_ids1 ->
+  AtomSetImpl.inter (ids2atoms ex_ids0) (codom rm1) [<=] {} ->
+  codom rm1 [<=] ids2atoms ex_ids1 ->
+  rm_codom_disjoint rm1 ->
+  dom rm1 [<=] ids2atoms ex_ids0 ->
+  gen_metadata_cmds nts ex_ids1 rm1 cs = Some (ex_ids2,rm2) ->
+  ids2atoms ex_ids1 [<=] ids2atoms ex_ids2 /\
+  AtomSetImpl.inter (ids2atoms ex_ids0) (codom rm2) [<=] {} /\
+  codom rm2 [<=] ids2atoms ex_ids2 /\
+  rm_codom_disjoint rm2 /\
+  dom rm2 [<=] ids2atoms ex_ids0.
+Proof.
+  induction cs; simpl; intros rm1 rm2 ex_ids1 ex_ids2 Hinc H1 H2 H3 H4 H6 H5.
+    inv H5. split; auto. fsetdec.
+
+    destruct (getCmdTyp nts a); tinv H5. simpl in H5.
+    assert ((getCmdLoc a) `in` ids2atoms ex_ids0) as Hin.
+      apply ids2atoms__inc in Hinc.
+      simpl in Hinc. fsetdec.
+    simpl_env in Hinc. apply incl_app_invr in Hinc.
+    destruct (isPointerTypB t).
+      case_eq (gen_metadata_id ex_ids1 rm1 (getCmdLoc a)).
+      intros [[b e] ex_ids5] rm5 Hgenid.
+      rewrite Hgenid in H5.
+      eapply gen_metadata_id_spec in Hgenid; eauto.
+      destruct Hgenid as [J8 [J9 [J10 [J11 J12]]]].
+      assert (ids2atoms ex_ids0[<=]ids2atoms ex_ids5) as Hinc'.
+        clear - H1 J8. fsetdec.
+      apply IHcs in H5; auto.
+      destruct H5 as [J1 [J2 [J3 J4]]].
+      split; auto. 
+         clear - J8 J1. fsetdec.
+
+      apply IHcs in H5; auto.
+Qed.
+
+Lemma gen_metadata_block_spec : forall nts ex_ids0 b rm1 rm2 ex_ids1 ex_ids2, 
+  incl (getBlockLocs b) ex_ids0 ->
+  ids2atoms ex_ids0 [<=] ids2atoms ex_ids1 ->
+  AtomSetImpl.inter (ids2atoms ex_ids0) (codom rm1) [<=] {} ->
+  codom rm1 [<=] ids2atoms ex_ids1 ->
+  rm_codom_disjoint rm1 ->
+  dom rm1 [<=] ids2atoms ex_ids0 ->
+  gen_metadata_block nts ex_ids1 rm1 b = Some (ex_ids2,rm2) ->
+  ids2atoms ex_ids1 [<=] ids2atoms ex_ids2 /\
+  AtomSetImpl.inter (ids2atoms ex_ids0) (codom rm2) [<=] {} /\
+  codom rm2 [<=] ids2atoms ex_ids2 /\
+  rm_codom_disjoint rm2 /\
+  dom rm2 [<=] ids2atoms ex_ids0.
+Proof.
+  intros nts ex_ids0 b rm1 rm2 ex_ids1 ex_ids2 Hinc H1 H2 H3 H4 H6 H5.
+  destruct b.
+  simpl in H5.
+  case_eq (gen_metadata_phinodes ex_ids1 rm1 p).
+  intros ex_ids5 rm5 Hgenps. rewrite Hgenps in H5.
+  simpl in Hinc.
+  assert (Hinc':=Hinc). 
+  apply incl_app_invl in Hinc'.
+  apply incl_app_invr in Hinc.
+  apply incl_app_invl in Hinc.
+  eapply gen_metadata_phinodes_spec in Hgenps; eauto.
+  destruct Hgenps as [J8 [J9 [J10 [J11 J12]]]].
+  assert (ids2atoms ex_ids0[<=]ids2atoms ex_ids5) as Hinc''.
+    clear - H1 J8. fsetdec.
+  eapply gen_metadata_cmds_spec in H5; eauto.
+  destruct H5 as [J1 [J2 [J3 [J4 J5]]]].
+  split; auto.
+    clear - J8 J1. fsetdec.
+Qed.
+
+Lemma gen_metadata_blocks_spec : forall nts ex_ids0 bs rm1 rm2 ex_ids1 ex_ids2, 
+  incl (getBlocksLocs bs) ex_ids0 ->
+  ids2atoms ex_ids0 [<=] ids2atoms ex_ids1 ->
+  AtomSetImpl.inter (ids2atoms ex_ids0) (codom rm1) [<=] {} ->
+  codom rm1 [<=] ids2atoms ex_ids1 ->
+  rm_codom_disjoint rm1 ->
+  dom rm1 [<=] ids2atoms ex_ids0 ->
+  gen_metadata_blocks nts ex_ids1 rm1 bs = Some (ex_ids2,rm2) ->
+  ids2atoms ex_ids1 [<=] ids2atoms ex_ids2 /\
+  AtomSetImpl.inter (ids2atoms ex_ids0) (codom rm2) [<=] {} /\
+  codom rm2 [<=] ids2atoms ex_ids2 /\
+  rm_codom_disjoint rm2 /\
+  dom rm2 [<=] ids2atoms ex_ids0.
+Proof.
+  induction bs; simpl; intros rm1 rm2 ex_ids1 ex_ids2 Hinc H1 H2 H3 H4 H6 H5.
+    inv H5. split; auto. fsetdec.
+
+    assert (Hinc':=Hinc). 
+    apply incl_app_invl in Hinc'.
+    apply incl_app_invr in Hinc.
+    remember (gen_metadata_block nts ex_ids1 rm1 a) as R.
+    destruct R as [[ex_ids5 rm5]|]; tinv H5.
+    symmetry in HeqR.
+    eapply gen_metadata_block_spec in HeqR; eauto.
+    destruct HeqR as [J8 [J9 [J10 [J11 J12]]]].
+    assert (ids2atoms ex_ids0[<=]ids2atoms ex_ids5) as Hinc''.
+      clear - H1 J8. fsetdec.
+    apply IHbs in H5; auto.
+    destruct H5 as [J1 [J2 [J3 J4]]].
+    split; auto. 
+       clear - J8 J1. fsetdec.
+Qed.
+    
+Lemma gen_metadata_fdef_spec : forall nts f1 rm2 ex_ids2,
+  gen_metadata_fdef nts (getFdefLocs f1) nil f1 = Some (ex_ids2,rm2) ->
+  ids2atoms (getFdefLocs f1) [<=] ids2atoms ex_ids2 /\
+  AtomSetImpl.inter (ids2atoms (getFdefLocs f1)) (codom rm2) [<=] {} /\
+  codom rm2 [<=] ids2atoms ex_ids2 /\
+  rm_codom_disjoint rm2.
+Proof.
+  intros nts f1 rm2 ex_ids2 Hgenf.
+  destruct f1. destruct f. simpl in *.
+  case_eq (gen_metadata_args (getArgsIDs a ++ getBlocksLocs b) nil a).
+  intros ex_ids3 rm3 Hgenargs.
+  rewrite Hgenargs in Hgenf.
+  assert (incl (getArgsIDs a) (getArgsIDs a ++ getBlocksLocs b)) as Hinc1.
+    apply incl_appl; auto using incl_refl.
+  assert (incl (getBlocksLocs b) (getArgsIDs a ++ getBlocksLocs b)) as Hinc2.
+    apply incl_appr; auto using incl_refl.
+  apply gen_metadata_args_spec with (ex_ids0:=getArgsIDs a ++ getBlocksLocs b) 
+    in Hgenargs; simpl; auto; try fsetdec.
+  destruct Hgenargs as [J1 [J2 [J3 [J4 J5]]]].
+  apply gen_metadata_blocks_spec with (ex_ids0:=getArgsIDs a ++ getBlocksLocs b) 
+    in Hgenf; auto.
+  destruct Hgenf as [J6 [J7 [J78 [J9 J10]]]].
+  split; auto.
+    fsetdec.
+Qed.
+
+Lemma reg_simulation__updateAddAL_lc : forall mi los nts gl f1 rm1 rm2 lc1 lc2 i0
+    gv gv' ex_ids3,
+  reg_simulation mi (los, nts) gl f1 rm1 rm2 lc1 lc2 ->
+  gen_metadata_fdef nts (getFdefLocs f1) nil f1 = Some (ex_ids3,rm2) ->
+  In i0 (getFdefLocs f1) ->
+  gv_inject mi gv gv' ->
+  reg_simulation mi (los, nts) gl f1 rm1 rm2 (updateAddAL GenericValue lc1 i0 gv)
+    (updateAddAL GenericValue lc2 i0 gv').
+Proof.
+  intros mi los nts gl f1 rm1 rm2 lc1 lc2 i0 gv gv' ex_ids3 Hsim Hgenmd Hin Hinj.
+
+  assert (Hspec := Hgenmd).
+  apply gen_metadata_fdef_spec in Hspec; auto.
+  destruct Hspec as [Hinc1 [Hdisj1 [Hinc3 Hdisj2]]].
+  clear Hinc1 Hinc3.
+  eapply ids2atoms_dom in Hin.
+  assert (i0 `notin` codom rm2) as Hnotin.
+    clear - Hin Hdisj1. fsetdec.
+
+  destruct Hsim as [J1 [J2 J3]].    
+  split.
+    intros i1 gv1 J.
+    destruct (id_dec i0 i1); subst.
+      rewrite lookupAL_updateAddAL_eq in *; auto.
+      inv J. exists gv'. auto.
+    
+      rewrite <- lookupAL_updateAddAL_neq in J; auto.
+      rewrite <- lookupAL_updateAddAL_neq; auto.
+
+  split.
+    intros vp bgv1 egv1 J.
+    apply J2 in J. 
+    destruct J as [bv2 [ev2 [bgv2 [egv2 [J11 [J12 [J13 [J14 J15]]]]]]]].
+    exists bv2. exists ev2. exists bgv2. exists egv2.
+    split; auto.
+    destruct vp as [pid |]; simpl in J11.
+      case_eq (lookupAL (id * id) rm2 pid).
+        intros [bid eid] J.
+        rewrite J in J11.    
+        inv J11.
+        simpl.
+        assert (J':=J).
+        apply in_codom_of_rmap in J'.    
+        destruct J' as [J16 J17].      
+        rewrite <- lookupAL_updateAddAL_neq; try solve [fsetdec].
+        rewrite <- lookupAL_updateAddAL_neq; try solve [fsetdec].
+        repeat (split; auto).
+
+        intro J.
+        rewrite J in J11. inversion J11.
+
+      case_eq (get_const_metadata c).
+        intros [bc ec] J.
+        rewrite J in J11.
+        inv J11.
+        simpl in *.
+        repeat (split; auto).
+
+        intro J.  rewrite J in J11.
+        inv J11. simpl in *.
+        repeat (split; auto).
+
+    intros i1 gv1 Hlk.
+    destruct (id_dec i0 i1); subst.
+      rewrite lookupAL_updateAddAL_eq in Hlk; auto.
+      inv Hlk. apply ids2atoms_dom in Hin; auto.
+    
+      rewrite <- lookupAL_updateAddAL_neq in Hlk; eauto.
+Qed.
+
+Lemma reg_simulation__updateAddAL_md : forall mi los nts gl f1 rm1 rm2 lc1 lc2 
+    id0 bgv1 bgv2 egv1 egv2 bid eid mgb M1 M2 ex_ids
   (Hwfmi : wf_sb_mi mgb mi M1 M2)
   (Hwfg : wf_globals mgb gl),
-  reg_simulation mi TD gl f1 rm1 rm2 lc1 lc2 ->
-  wf_fresh ex_ids3 c rm2 ->
-  getCmdID c = Some id0 ->
+  gen_metadata_fdef nts (getFdefLocs f1) nil f1 = Some (ex_ids,rm2) ->
+  reg_simulation mi (los,nts) gl f1 rm1 rm2 lc1 lc2 ->
   ret (bid, eid) = lookupAL (id * id) rm2 id0 ->
   gv_inject mi bgv1 bgv2 ->
   gv_inject mi egv1 egv2 ->
-  reg_simulation mi TD gl f1 
+  reg_simulation mi (los,nts) gl f1 
     (updateAddAL _ rm1 id0 (mkMD bgv1 egv1)) rm2 lc1
     (updateAddAL _ (updateAddAL _ lc2 bid bgv2) eid egv2).
 Proof.
-  intros mi TD gl f1 rm1 rm2 lc1 lc2 id0 bgv1 bgv2 egv1 egv2 bid eid c ex_ids3
-    mgb M1 M2 Hwfmi Hwfg Hrsim Hnotin Hid HeqR1 Hbinj Heinj.
+  intros mi los nts gl f1 rm1 rm2 lc1 lc2 id0 bgv1 bgv2 egv1 egv2 bid eid mgb M1 
+    M2 ex_ids Hwfmi Hwfg Hgenmd Hrsim HeqR1 Hbinj Heinj.
+  assert (Hspec := Hgenmd).
+  apply gen_metadata_fdef_spec in Hspec; auto.
+  destruct Hspec as [Hinc1 [Hdisj1 [Hinc3 Hdisj2]]].
+  clear Hinc1 Hinc3.
   split.
   SSCase "rsim1".
       intros i0 gv1 J.
+      assert (Hin:=Hrsim).
+      eapply reg_simulation_spec in Hin; eauto.
+      
       destruct Hrsim as [J1 _].
       apply J1 in J.
-      destruct J as [gv2 [J J2]].
+      destruct J as [gv2 [J2 J3]].
       exists gv2.
         split; auto.
-          admit. (* i0 <> bid eid tmp, need to fix simulation relation for 
-                    freshness *)
+        apply notin_codom__neq with (id0:=i0)(id1:=id0)(bid:=bid)(eid:=eid)
+          (rm:=rm2)(d:=ids2atoms (getFdefLocs f1)) in Hdisj1; auto.
+        destruct Hdisj1 as [Heq1 Heq2].
+        rewrite <- lookupAL_updateAddAL_neq; auto.
+        rewrite <- lookupAL_updateAddAL_neq; auto.
+
+  split.
   SSCase "rsim2".
       intros vp bgv0 egv0 J.
       unfold SBopsem.get_reg_metadata in J.
@@ -2586,21 +1137,17 @@ Proof.
           exists bgv2. exists egv2.
           split; auto.
           split.
-            clear - Hnotin HeqR1.
-            destruct Hnotin as [Hnotin1 [Hnotin2 [Hnotin3 Hnotin4]]]. 
-            unfold getCmdIDs in *.
             simpl in *.
-            simpl.
             rewrite <- lookupAL_updateAddAL_neq.
               rewrite lookupAL_updateAddAL_eq; auto.
-              eapply rm_codom_disjoint_spec in HeqR1; eauto.
+              eapply rm_codom_disjoint_spec in HeqR1; eauto. 
 
           split. simpl. rewrite lookupAL_updateAddAL_eq; auto.
           split; auto.
 
         SSSSCase "id0 <> pid".
           rewrite <- lookupAL_updateAddAL_neq in J; auto.
-          destruct Hrsim as [_ Hrsim].
+          destruct Hrsim as [_ [Hrsim _]].
           destruct (@Hrsim (value_id pid) bgv0 egv0) as 
             [bv2 [ev2 [bgv2' [egv2' [J1 [J2 [J3 [J4 J5]]]]]]]]; auto.
           exists bv2. exists ev2. exists bgv2'. exists egv2'.
@@ -2608,10 +1155,10 @@ Proof.
           split; auto.
           remember (lookupAL (id * id) rm2 pid) as R.
           destruct R; inv J1. destruct p; inv H0.
-          destruct Hnotin as [Hnotin1 [Hnotin2 [Hnotin3 Hnotin4]]]. 
-          eapply rm_codom_disjoint_spec' with (id1:=id0)(id2:=pid) in Hnotin4; 
+          simpl.
+          eapply rm_codom_disjoint_spec' with (id1:=id0)(id2:=pid) in Hdisj2; 
             eauto.
-          destruct Hnotin4 as [G1 [G2 [G3 [G4 [G5 [G6 [G7 [G8 [G9 G10]]]]]]]]]. 
+          destruct Hdisj2 as [G1 [G2 [G3 [G4 [G5 [G6 [G7 [G8 [G9 G10]]]]]]]]]. 
           simpl.
           split.
             rewrite <- lookupAL_updateAddAL_neq; auto.
@@ -2620,11 +1167,11 @@ Proof.
             rewrite <- lookupAL_updateAddAL_neq; auto.
 
       SSSCase "vp = c".
-        remember (get_const_metadata c0) as R.
+        remember (get_const_metadata c) as R.
         destruct R as [[c1 c2]|].
-          remember (const2GV TD gl c1) as R1.
+          remember (const2GV (los,nts) gl c1) as R1.
           destruct R1; try solve [inversion J]. simpl in J.
-          remember (const2GV TD gl c2) as R2.
+          remember (const2GV (los,nts) gl c2) as R2.
           destruct R2; try solve [inversion J]. simpl in J.
           inv J.
           exists (value_const c1). exists (value_const c2). simpl.
@@ -2637,37 +1184,133 @@ Proof.
           unfold val2GV.
           inv Hwfmi.
           repeat (split; eauto).
+
+  SSCase "rsim3".
+    destruct Hrsim as [_ [_ Hrsim]]; auto.
 Qed.
 
+Lemma tmp_is_fresh2 : forall i0 d tmp ex_ids' ex_ids1 ex_ids2,
+  In i0 d ->
+  ids2atoms d [<=] ids2atoms ex_ids1 ->
+  incl ex_ids1 ex_ids2 ->
+  (tmp, ex_ids') = mk_tmp ex_ids2 ->
+  i0 <> tmp.
+Proof.
+  intros.
+  apply ids2atoms__inc in H1.
+  apply ids2atoms__in in H.
+  eapply tmp_is_fresh with (ex_ids:=ex_ids2); eauto.
+    fsetdec.
+Qed. 
 
-Lemma reg_simulation__updateAddAL_tmp : forall mi TD gl f1 rm1 rm2 lc1 lc2 tmp
-   tgv c ex_ids3 ex_ids5 mgb M1 M2
+Lemma tmp_is_fresh3 : forall ex_ids1 ex_ids2 tmp ex_ids' bid eid rm id1,
+  codom rm [<=] ids2atoms ex_ids1 ->
+  Some (bid, eid) = lookupAL _ rm id1 ->
+  incl ex_ids1 ex_ids2 ->
+  (tmp, ex_ids') = mk_tmp ex_ids2 ->
+  bid <> tmp /\ eid <> tmp.
+Proof.
+  intros.
+  apply ids2atoms__inc in H1.
+  eapply tmp_is_fresh' with (ex_ids:=ex_ids2); eauto.
+    fsetdec.
+Qed. 
+
+Lemma get_reg_metadata_fresh'' : forall
+  (rm2 : rmap)
+  (ex_ids : ids)
+  (id0 : id) f1 nts
+  (Hgenmd : gen_metadata_fdef nts (getFdefLocs f1) nil f1 = Some (ex_ids,rm2))
+  (Hin : In id0 (getFdefLocs f1))
+  (vp0 : value)
+  (bv0 : value)
+  (ev0 : value)
+  (J11 : get_reg_metadata rm2 vp0 = ret (bv0, ev0)),
+  id_fresh_in_value bv0 id0 /\ id_fresh_in_value ev0 id0.
+Proof.
+  intros.
+  apply gen_metadata_fdef_spec in Hgenmd; auto.
+  destruct Hgenmd as [Hinc1 [Hdisj1 [Hinc3 Hdisj2]]].
+  clear Hinc1 Hinc3 Hdisj2.
+  destruct vp0; simpl in J11.
+    remember (lookupAL (id * id) rm2 i0) as R.
+    destruct R as [[bid eid]|]; inv J11.
+    simpl.
+    apply rmap_lookupAL in HeqR.
+    destruct HeqR as [J1 [J2 _]].
+    apply ids2atoms__in in Hin.
+    clear - Hdisj1 Hin J1 J2.
+    fsetdec.
+  
+    destruct (SBopsem.get_const_metadata c) as [[be ec]|]; inv J11; simpl; auto.
+Qed.
+
+Lemma get_reg_metadata_fresh3 : forall nts f1 ex_ids3 rm2 vp bv2 ev2 id0 bid0
+    eid0,
+  gen_metadata_fdef nts (getFdefLocs f1) nil f1 = Some (ex_ids3,rm2) ->
+  get_reg_metadata rm2 vp = ret (bv2, ev2) ->
+  lookupAL (id * id) rm2 id0 = ret (bid0, eid0) ->
+  id_fresh_in_value ev2 bid0 /\ id_fresh_in_value bv2 eid0.
+Proof.
+  intros nts f1 ex_ids3 rm2 vp bv2 ev2 id0 bid0 eid0 Hgenmd Hgetr Hlk.
+  apply gen_metadata_fdef_spec in Hgenmd; auto.
+  destruct Hgenmd as [Hinc1 [Hdisj1 [Hinc3 Hdisj2]]].
+  clear Hinc1 Hinc3 Hdisj1.
+  destruct vp; simpl in Hgetr.
+    remember (lookupAL (id * id) rm2 i0) as R.
+    destruct R as [[bid eid]|]; inv Hgetr.
+    simpl. symmetry in Hlk. 
+    destruct (i0==id0); subst.
+      rewrite <- Hlk in HeqR. inv HeqR.
+      apply rm_codom_disjoint_spec in Hlk; auto.
+      destruct Hlk as [J1 [J2 _]]. auto.
+
+      apply rm_codom_disjoint_spec' with (id1:=id0)(bid1:=bid0)(eid1:=eid0) 
+        in HeqR; auto.
+      destruct HeqR as [G1 [G2 [G3 [G4 [G5 [G6 [G7 [G8 [G9 G10]]]]]]]]]. 
+      auto.
+  
+    destruct (SBopsem.get_const_metadata c) as [[be ec]|]; 
+      inv Hgetr; simpl; auto.
+Qed.        
+
+Lemma reg_simulation__updateAddAL_tmp : forall mi los nts gl f1 rm1 rm2 lc1 lc2 
+   tmp tgv ex_ids3 ex_ids3' ex_ids5 mgb M1 M2
   (Hwfmi : wf_sb_mi mgb mi M1 M2)
   (Hwfg : wf_globals mgb gl),
-  reg_simulation mi TD gl f1 rm1 rm2 lc1 lc2 ->
-  wf_fresh ex_ids3 c rm2 ->
-  (tmp, ex_ids5) = mk_tmp ex_ids3 ->
-  reg_simulation mi TD gl f1 rm1 rm2 lc1 (updateAddAL _ lc2 tmp tgv).
+  reg_simulation mi (los, nts) gl f1 rm1 rm2 lc1 lc2 ->
+  gen_metadata_fdef nts (getFdefLocs f1) nil f1 = Some (ex_ids3,rm2) ->
+  incl ex_ids3 ex_ids3' ->
+  (tmp, ex_ids5) = mk_tmp ex_ids3' ->
+  reg_simulation mi (los, nts) gl f1 rm1 rm2 lc1 (updateAddAL _ lc2 tmp tgv).
 Proof.
-  intros mi TD gl f1 rm1 rm2 lc1 lc2 tmp tgv c ex_ids3 ex_ids5 mgb M1 M2 Hwfmi 
-    Hwfg Hrsim Hnotin HeqR2.
+  intros mi los nts gl f1 rm1 rm2 lc1 lc2 tmp tgv ex_ids3 ex_ids3' ex_ids5 mgb M1
+    M2 Hwfmi Hwfg Hrsim Hgenmd Htmp HeqR2.
+  assert (Hspec := Hgenmd).
+  apply gen_metadata_fdef_spec in Hspec; auto.
+  destruct Hspec as [Hinc1 [Hdisj1 [Hinc3 Hdisj2]]].
+  clear Hdisj1.
     split.
     SSCase "rsim1".
       intros i0 gv1 J.
+      assert (Hin:=Hrsim).
+      eapply reg_simulation_spec in Hin; eauto.
       destruct Hrsim as [J1 _].
       apply J1 in J.
       destruct J as [gv2 [J J2]].
       exists gv2.
       split; auto.
-        admit. (* i0 <> bid eid tmp, need to fix simulation relation for 
-                    freshness *)
- 
+        eapply tmp_is_fresh2 in Hinc1; eauto.
+        rewrite <- lookupAL_updateAddAL_neq; auto.
+          apply ids2atoms__in. apply in_singleton; auto.
+
+    split.
     SSCase "rsim2".
       intros vp bgv1 egv1 J.
       unfold SBopsem.get_reg_metadata in J.
       destruct vp as [pid | ]; simpl.
       SSSCase "vp = pid".
-          destruct Hrsim as [_ Hrsim].
+          destruct Hrsim as [_ [Hrsim _]].
           destruct (@Hrsim (value_id pid) bgv1 egv1) as 
             [bv2 [ev2 [bgv2 [egv2 [J1 [J2 [J3 [J4 J5]]]]]]]]; auto.
           exists bv2. exists ev2. exists bgv2. exists egv2.
@@ -2675,21 +1318,18 @@ Proof.
           split; auto.
           remember (lookupAL (id * id) rm2 pid) as R.
           destruct R; inv J1. destruct p; inv H0.
-          destruct Hnotin as [Hnotin1 [Hnotin2 [Hnotin3 Hnotin4]]]. 
+          eapply tmp_is_fresh3 in HeqR; eauto.
+          destruct HeqR as [Hneq1 Hneq2]. 
           simpl.
           rewrite <- lookupAL_updateAddAL_neq; auto.
           rewrite <- lookupAL_updateAddAL_neq; auto.
-            eapply tmp_is_fresh' with (tmp:=tmp) in HeqR; eauto. 
-              clear - Hnotin3. fsetdec.
-            eapply tmp_is_fresh' with (tmp:=tmp) in HeqR; eauto. 
-              clear - Hnotin3. fsetdec.
 
       SSSCase "vp = c".
-        remember (get_const_metadata c0) as R.
+        remember (get_const_metadata c) as R.
         destruct R as [[c1 c2]|].
-          remember (const2GV TD gl c1) as R1.
+          remember (const2GV (los, nts) gl c1) as R1.
           destruct R1; try solve [inversion J]. simpl in J.
-          remember (const2GV TD gl c2) as R2.
+          remember (const2GV (los, nts) gl c2) as R2.
           destruct R2; try solve [inversion J]. simpl in J.
           inv J.
           exists (value_const c1). exists (value_const c2). simpl.
@@ -2702,6 +1342,8 @@ Proof.
           unfold val2GV.
           inv Hwfmi.
           repeat (split; eauto).
+
+    SSCase "rsim3". destruct Hrsim as [_ [_ Hrsim]]; auto.
 Qed.
 
 Lemma mem_simulation__free : forall mi TD MM Mem0 M2 Mem' mgb hi lo
@@ -2855,7 +1497,7 @@ Proof.
   destruct c; try solve [inv H0].
   destruct H0 as [J0 [J1 [J2 [Htfdef [Heq0 [Hasim [Hnth [Heqb1 [Heqb2 [ex_ids 
     [rm2 [ex_ids3 [ex_ids4 [cs22 [cs23 [cs24 [Hgenmeta [Hrsim [Hinc [Hcall 
-    [Hfresh [Htcmds [Httmn Heq2]]]]]]]]]]]]]]]]]]]]]]]; subst.
+    [Htcmds [Httmn Heq2]]]]]]]]]]]]]]]]]]]]]]; subst.
   eapply inject_incr__preserves__als_simulation in Hasim; eauto.
   eapply inject_incr__preserves__reg_simulation in Hrsim; eauto.
   repeat (split; auto).
@@ -2885,20 +1527,18 @@ Proof.
   exists l1. exists ps1. exists (cs11 ++ [c]). simpl_env. auto.
 Qed.
 
-Lemma reg_simulation__updateAddAL_prop : forall mi TD gl f1 rm1 rm2 lc1 lc2  
-    bgv1 bgv2 egv1 egv2 bid eid c ex_ids3 mgb M1 M2 id0 gv1 gv2
+Lemma reg_simulation__updateAddAL_prop : forall mi los nts gl f1 rm1 rm2 lc1 lc2 
+    bgv1 bgv2 egv1 egv2 bid eid ex_ids3 mgb M1 M2 id0 gv1 gv2
   (Hwfmi : wf_sb_mi mgb mi M1 M2)
   (Hwfg : wf_globals mgb gl),
-  reg_simulation mi TD gl f1 rm1 rm2 lc1 lc2 ->
-  wf_fresh ex_ids3 c rm2 ->
-  getCmdID c = Some id0 ->
+  gen_metadata_fdef nts (getFdefLocs f1) nil f1 = Some (ex_ids3,rm2) ->
+  reg_simulation mi (los,nts) gl f1 rm1 rm2 lc1 lc2 ->
   ret (bid, eid) = lookupAL (id * id) rm2 id0 ->
   In id0 (getFdefLocs f1) ->
-  id0 `notin` codom rm2 ->
   gv_inject mi gv1 gv2 ->
   gv_inject mi bgv1 bgv2 ->
   gv_inject mi egv1 egv2 ->
-  reg_simulation mi TD gl f1 
+  reg_simulation mi (los,nts)  gl f1 
     (updateAddAL _ rm1 id0 (mkMD bgv1 egv1)) rm2 
     (updateAddAL GenericValue lc1 id0 gv1)
     (updateAddAL _ (updateAddAL _ 
@@ -2908,7 +1548,6 @@ Proof.
   eapply reg_simulation__updateAddAL_md; eauto.
   eapply reg_simulation__updateAddAL_lc; eauto.
 Qed.
-
 
 Lemma simulation__mload : forall mi TD MM Mem0 Mem2 gvp align0 gv t gvp2 mgb,
   wf_sb_mi mgb mi Mem0 Mem2 ->
@@ -2953,7 +1592,7 @@ Proof.
       inversion_clear Hwfmi.
       apply mi_range_block in H2. subst.
       rewrite Int.add_zero.
-      assert (Int.signed 31 i1 + 0 = Int.signed 31 i1) as EQ. zauto.
+      assert (Int.signed 31 i2 + 0 = Int.signed 31 i2) as EQ. zauto.
       rewrite EQ in J2. rewrite J2. auto.
 
       unfold val2GV. simpl. 
@@ -2962,49 +1601,47 @@ Proof.
     destruct p. simpl in HeqR3. destruct (split gvp2). inversion HeqR3.
 Qed.
 
-
 Lemma get_reg_metadata__fresh : forall
-  (rm2 : rmap)
-  (ex_ids : ids)
-  c
-  (Hnotin : wf_fresh ex_ids c rm2)
-  (t2 : typ)
-  (bv2 : value)
-  (ev2 : value)
-  (ptmp : id)
-  (ex_ids1 : ids)
+  (rm2 : rmap) (ex_ids ex_ids1 ex_ids3: ids) (bv2 ev2 : value) (ptmp : id) f1 nts
+  (Hgenmd : gen_metadata_fdef nts (getFdefLocs f1) nil f1 = Some (ex_ids3,rm2))
+  (Hinc : incl ex_ids3 ex_ids) vp
   (HeqR1 : (ptmp, ex_ids1) = mk_tmp ex_ids)
-  vp
   (J1 : SB_ds_pass.get_reg_metadata rm2 vp = ret (bv2, ev2)),
   id_fresh_in_value bv2 ptmp /\ id_fresh_in_value ev2 ptmp.
 Proof.
   intros.
+  apply gen_metadata_fdef_spec in Hgenmd; auto.
+  destruct Hgenmd as [Hinc1 [Hdisj1 [Hinc3 Hdisj2]]].
+  clear Hinc1 Hdisj2.
   destruct vp; simpl in *.
   remember (lookupAL (id * id) rm2 i0) as R.
   destruct R; inv J1.
   destruct p; inv H0; simpl.
-  destruct Hnotin as [_ [_ [Hnotin _ ]]].
-  eapply tmp_is_fresh' with (tmp:=ptmp) in HeqR; eauto. fsetdec.
-  
-  destruct (SBopsem.get_const_metadata c0) as [[bc ec]|].
-    inv J1; simpl; auto.
-    destruct (Constant.getTyp c0); inv J1; simpl; auto.
+  apply ids2atoms__inc in Hinc.
+  eapply tmp_is_fresh' with (tmp:=ptmp)(ex_ids:=ex_ids) in HeqR; eauto. 
+    fsetdec.
+  destruct (SBopsem.get_const_metadata c) as [[bc ec]|]; inv J1; simpl; auto.
 Qed.            
 
-Lemma get_reg_metadata_fresh' : forall vp rm2 ex_ids
-  (Hnotin1 : AtomSetImpl.inter (getValueID vp) (codom rm2)[<=]empty)
-  (Hnotin2 : union (getValueID vp) (codom rm2)[<=] ids2atoms ex_ids)
+Lemma get_reg_metadata_fresh' : forall nts vp rm2 ex_ids3 f1
+  (Hgenmd : gen_metadata_fdef nts (getFdefLocs f1) nil f1 = Some (ex_ids3,rm2))
+  (Hnotin : (getValueID vp) [<=] ids2atoms ((getFdefLocs f1)))
   (ptmp : id)
-  (ex_ids1 : ids)
+  (ex_ids1 ex_ids: ids)
+  (Hinc : incl ex_ids3 ex_ids)
   (HeqR1 : (ptmp, ex_ids1) = mk_tmp ex_ids),
   id_fresh_in_value vp ptmp.
 Proof.
   intros.
+  apply gen_metadata_fdef_spec in Hgenmd; auto.
+  destruct Hgenmd as [Hinc1 [Hdisj1 [Hinc3 Hdisj2]]].
+  clear Hdisj2.
   destruct vp; simpl in *; auto.
     apply tmp_is_fresh with (i0:=i0)(d:=singleton i0) in HeqR1; auto.
-      clear - Hnotin2. fsetdec.
+      apply ids2atoms__inc in Hinc.
+      fsetdec.
 Qed.
-
+(*
 Lemma wf_fresh__mk_tmp' : forall ex_ids vp rm2 ptmp ex_ids1,
  union (getValueID vp) (codom rm2)[<=] ids2atoms ex_ids ->
  (ptmp, ex_ids1) = mk_tmp ex_ids ->
@@ -3020,7 +1657,6 @@ Proof.
       apply ids2atoms_dom; auto.              
     fsetdec.
 Qed.
-
 Lemma get_reg_metadata_fresh'' : forall
   (rm2 : rmap)
   (ex_ids : ids)
@@ -3051,56 +1687,7 @@ Proof.
       inv J11; simpl; auto.
       destruct (Constant.getTyp c); inv J11; simpl; auto.
 Qed.
-
-Axiom store_doesnt_change_gmmd : forall M2 b2 ofs v0 Mem2' lc2 gl als
-   bid0 eid0 bgv' egv' fs F B cs tmn S Ps EC TD v ck,
-  Mem.store ck M2 b2 ofs v0 = ret Mem2' ->
-  LLVMopsem.dsop_star 
-    (LLVMopsem.mkState S TD Ps 
-      ((LLVMopsem.mkEC F B 
-        (insn_call bid0 false attrs gmb_typ gmb_fn 
-                       ((p8,v)::
-                        (p8,vnullp8)::
-                        (i32,vint1)::
-                        (p32,vnullp32)::
-                        nil)::
-         insn_call eid0 false attrs gme_typ gme_fn 
-                       ((p8,v)::
-                        (p8,vnullp8)::
-                        (i32,vint1)::
-                        (p32,vnullp32)::
-                        nil)::
-         cs) 
-        tmn lc2 als)
-        ::EC) gl fs M2)
-    (LLVMopsem.mkState S TD Ps 
-       ((LLVMopsem.mkEC F B cs tmn 
-         (updateAddAL _ (updateAddAL _ lc2 bid0 bgv') eid0 egv') als)::EC) 
-        gl fs M2)
-    trace_nil ->
-  LLVMopsem.dsop_star 
-    (LLVMopsem.mkState S TD Ps 
-      ((LLVMopsem.mkEC F B 
-        (insn_call bid0 false attrs gmb_typ gmb_fn 
-                       ((p8,v)::
-                        (p8,vnullp8)::
-                        (i32,vint1)::
-                        (p32,vnullp32)::
-                        nil)::
-         insn_call eid0 false attrs gme_typ gme_fn 
-                       ((p8,v)::
-                        (p8,vnullp8)::
-                        (i32,vint1)::
-                        (p32,vnullp32)::
-                        nil)::
-         cs) 
-        tmn lc2 als)
-        ::EC) gl fs Mem2')
-    (LLVMopsem.mkState S TD Ps 
-       ((LLVMopsem.mkEC F B cs tmn 
-         (updateAddAL _ (updateAddAL _ lc2 bid0 bgv') eid0 egv') als)::EC) 
-        gl fs Mem2')
-    trace_nil.
+*)
 
 Lemma simulation__mstore : forall mi TD MM Mem0 Mem2 gvp align0 gv t gvp2 gv2
                                   Mem0' mgb,
@@ -3180,14 +1767,14 @@ Proof.
     destruct H0 as [Mem2' [J2 J4]].
     exists Mem2'.
     assert ( mstore TD Mem2
-      ((Vptr b2 (Int.add 31 i1 (Int.repr 31 delta)), m1) :: nil) t
+      ((Vptr b2 (Int.add 31 i2 (Int.repr 31 delta)), m1) :: nil) t
       gv2 align0 = ret Mem2') as J.
       unfold mstore. simpl. rewrite <- HeqR'. rewrite Hg2v.
       clear - J2 Hwfmi H2.
       inversion_clear Hwfmi.
       apply mi_range_block in H2. subst.
       rewrite Int.add_zero.
-      assert (Int.signed 31 i1 + 0 = Int.signed 31 i1) as EQ. zauto.
+      assert (Int.signed 31 i2 + 0 = Int.signed 31 i2) as EQ. zauto.
       rewrite EQ in J2. auto.
     split; auto.
     split.
@@ -3246,7 +1833,7 @@ Proof.
   destruct p.
   destruct v; try solve [inversion HeqR].
   destruct gvp2; inv HeqR.
-  exists b0. exists i1. 
+  exists b0. exists i2. 
   unfold ptr2GV, val2GV. eauto.
 Qed.
 
@@ -3282,7 +1869,7 @@ Proof.
   destruct p.
   destruct v; try solve [inversion HeqR].
   destruct gvp2; inv HeqR.
-  exists b0. exists i1.  eauto.
+  exists b0. exists i2. eauto.
 Qed.
 
 Lemma prop_metadata_inv : forall ex_ids3 rm2 c vp id0 ex_ids5 cs1',
@@ -3300,63 +1887,6 @@ Proof.
   destruct (lookupAL _ rm2 id0) as [[bid0 eid0]|]; inv H.
   exists bv. exists ev. exists bid0. exists eid0. split; auto.
 Qed.
-
-Lemma defined_gv_dec : forall gv, defined_gv gv \/ ~ defined_gv gv.
-Proof.
-  destruct gv; simpl; auto.
-    destruct p; simpl; auto.
-    destruct v; simpl; try solve [left; congruence].
-      right. intro J. contradict J; auto.
-Qed.      
-
-Lemma defined_gvs_dec : forall gvs, defined_gvs gvs \/ ~ defined_gvs gvs.
-Proof.
-  induction gvs; simpl; auto.
-    destruct IHgvs as [IHgvs | IHgvs].
-      destruct (@defined_gv_dec a) as [J | J]; auto.
-        right. intros [J1 J2]. congruence.
-      right. intros [J1 J2]. congruence.
-Qed.
-
-Lemma memory_chuck_dec : forall (mc1 mc2:AST.memory_chunk), 
-  mc1 = mc2 \/ mc1 <> mc2.
-Proof.
-  destruct mc1; destruct mc2; try solve [auto | right; congruence].
-    destruct (eq_nat_dec n n0); auto.
-      right. intros J. inv J. auto.
-Qed.
-
-Lemma chunk_matched_dec : forall gv1 gv2, 
-  chunk_matched gv1 gv2 \/ ~ chunk_matched gv1 gv2.
-Proof.
-  induction gv1; destruct gv2.
-    left. apply chunk_matched_nil_refl.
-    right. intro J. apply chunk_matched_nil_inv in J. inv J.
-
-    right. intro J. apply chunk_matched_nil_inv' in J. inv J.
-    destruct a. destruct p.
-    destruct (@memory_chuck_dec m m0) as [J | J]; subst.
-      destruct (@IHgv1 gv2) as [J' | J'].
-        left. apply chunk_matched_cons_intro; auto.
-        right. intro J. apply chunk_matched_cons_inv in J.
-          destruct J as [gv2' [v1 [m1 [v2 [J1 [J2 J3]]]]]].
-          inv J3. inv J1. congruence.
-      right. intro J1. apply chunk_matched_cons_inv in J1.
-        destruct J1 as [gv2' [v1 [m1 [v2 [J1 [J2 J3]]]]]].
-        inv J3. inv J1. congruence.
-Qed.     
-
-Lemma gv_inject_null_refl : forall mgb mi M1 M2,
-  wf_sb_mi mgb mi M1 M2 -> gv_inject mi null null.
-Proof.
-  intros. inv H. unfold gv_inject. simpl. eauto.
-Qed.
-
-Lemma incl_cons : forall A l1 (x:A), incl l1 (x::l1).
-Proof.
-  intros. intros y J. simpl; auto.
-Qed.
-
 
 Lemma prop_metadata_mono : forall ex_ids1 rm c v i0 ex_ids2 cs2,
   prop_metadata ex_ids1 rm c v i0 =  ret (ex_ids2, cs2) ->
@@ -3382,16 +1912,26 @@ Proof.
   
     destruct (lookupAL (id * id) rm i0) as [[bid eid]|]; inv H.
     remember (mk_tmp ex_ids1) as R.
+    destruct R; tinv H1.
+    remember (mk_tmp i3) as R.
     destruct R; inv H1.
-    unfold mk_tmp in HeqR.
-    destruct (atom_fresh_for_list ex_ids1); inv HeqR; auto using incl_cons.
+    unfold mk_tmp in *.
+    destruct (atom_fresh_for_list ex_ids1); inv HeqR.
+    destruct (atom_fresh_for_list (x::ex_ids1)); inv HeqR0.
+    simpl_env.
+    apply incl_appr. apply incl_appr. apply incl_refl.
 
     destruct (lookupAL (id * id) rm i0) as [[bid eid]|]; inv H.
     remember (mk_tmp ex_ids1) as R.
+    destruct R; tinv H1.
+    remember (mk_tmp i3) as R.
     destruct R; inv H1.
-    unfold mk_tmp in HeqR.
-    destruct (atom_fresh_for_list ex_ids1); inv HeqR; auto using incl_cons.
-    
+    unfold mk_tmp in *.
+    destruct (atom_fresh_for_list ex_ids1); inv HeqR.
+    destruct (atom_fresh_for_list (x::ex_ids1)); inv HeqR0.
+    simpl_env.
+    apply incl_appr. apply incl_appr. apply incl_refl.
+
     destruct (get_reg_metadata rm v) as [[? ?]|]; try solve [inv H].
     remember (mk_tmp ex_ids1) as R.
     destruct R; inv H.
@@ -3426,7 +1966,10 @@ Proof.
       destruct (get_reg_metadata rm v0) as [[? ?]|]; inv H.
       destruct (get_reg_metadata rm v1) as [[? ?]|]; inv H1.
       destruct (lookupAL (id * id) rm i0) as [[? ?]|]; inv H0.
-        auto using incl_refl.
+      unfold mk_tmp in H1.
+      destruct (atom_fresh_for_list ex_ids1); inv H1.
+      auto using incl_cons.
+
       inv H. auto using incl_refl.
 
     destruct (trans_params rm p 1) as [?|]; inv H.
@@ -3522,8 +2065,7 @@ Proof.
   destruct (isCallLib fid).
     inv H; auto.
 
-    destruct (gen_metadata_args (let '(_, ids0) := split la in
-               ids0 ++ getBlocksLocs bs) nil la).
+    destruct (gen_metadata_args (getArgsIDs la ++ getBlocksLocs bs) nil la).
     destruct (gen_metadata_blocks nts i0 r bs) as [[ex_ids rm]|]; inv H.
     exists ex_ids. exists rm.
     destruct (trans_args rm la 1) as [cs'|]; inv H1.
@@ -3532,7 +2074,7 @@ Proof.
     destruct p.
     destruct b; inv H1.
     destruct b; inv H0. 
-    exists i1. exists b0. exists l0. exists p. exists c. exists t0.
+    exists i2. exists b0. exists l0. exists p. exists c. exists t0.
     eauto.
 Qed.
 
@@ -3582,7 +2124,6 @@ Proof.
       eapply incl_tran; eauto.
 Qed.
 
-
 Lemma wrapper_is_identical : forall fv, wrap_call fv = fv.
 Proof. 
   unfold wrap_call. 
@@ -3590,7 +2131,6 @@ Proof.
   destruct c; auto. 
     rewrite wrapper_fid_is_identical. auto.
 Qed.
-
 
 Lemma trans_products__trans_fdef : forall nts Ps1 Ps2 fid f1,
   trans_products nts Ps1 = Some Ps2 ->
@@ -3708,7 +2248,6 @@ Proof.
      simpl. eauto.
 Qed.
 
-
 Lemma trans_products__trans_fdec : forall nts Ps1 Ps2 fid f1,
   trans_products nts Ps1 = Some Ps2 ->
   lookupFdecViaIDFromProducts Ps1 fid = ret f1 ->
@@ -3739,7 +2278,6 @@ Proof.
       destruct R; inv HeqR.
       simpl. eauto.
 Qed.
-
 
 Lemma trans_products__none : forall nts Ps1 Ps2 fid,
   trans_products nts Ps1 = Some Ps2 ->
@@ -3808,7 +2346,8 @@ Proof.
   erewrite trans_products__none; eauto.
   eapply trans_products__trans_fdec; eauto.
 Qed.
-  Lemma getValueViaBlockFromValuels__eql : forall B1 B2 vls,
+
+Lemma getValueViaBlockFromValuels__eql : forall B1 B2 vls,
   label_of_block B1 = label_of_block B2 ->
   getValueViaBlockFromValuels vls B1 = getValueViaBlockFromValuels vls B2.
 Proof.
@@ -3923,49 +2462,43 @@ Proof.
       repeat (split; auto). 
 Qed.
 
-Lemma reg_simulation__updateAddAL_prop' : forall mi TD gl f1 rm1 rm2 lc1 lc2  
-    bgv1 bgv2 egv1 egv2 bid eid mgb M1 M2 id0 gv1 gv2
-  (Hwfmi : wf_sb_mi mgb mi M1 M2)
-  (Hwfg : wf_globals mgb gl),
-  reg_simulation mi TD gl f1 rm1 rm2 lc1 lc2 ->
-  ret (bid, eid) = lookupAL (id * id) rm2 id0 ->
-  gv_inject mi gv1 gv2 ->
-  gv_inject mi bgv1 bgv2 ->
-  gv_inject mi egv1 egv2 ->
-  reg_simulation mi TD gl f1 
-    (updateAddAL _ rm1 id0 (mkMD bgv1 egv1)) rm2 
-    (updateAddAL GenericValue lc1 id0 gv1)
-    (updateAddAL _ (updateAddAL _ 
-      (updateAddAL GenericValue lc2 id0 gv2) bid bgv2) eid egv2).
-Admitted. (*fresh*)
+Fixpoint incomingValues_in_dom (re1:list (id * GenericValue * monad metadata)) 
+  (d:ids) : Prop :=
+match re1 with
+| nil => True
+| (id1,_,_)::re1' => In id1 d /\ incomingValues_in_dom re1' d 
+end.
 
-Lemma updateValuesForNewBlock__reg_simulation : forall mi TD gl F rm2 re1 rm1 lc1
-    lc2 re2 lc1' rm1' lc2' M1 M2 mgb 
+Lemma updateValuesForNewBlock__reg_simulation : forall mi los gl f1 rm2 re1 
+    rm1 lc1 lc2 re2 lc1' rm1' lc2' M1 M2 mgb ex_ids nts
   (Hwfmi : wf_sb_mi mgb mi M1 M2)
   (Hwfg : wf_globals mgb gl),
-  reg_simulation mi TD gl F rm1 rm2 lc1 lc2 ->
+  incomingValues_in_dom re1 (getFdefLocs f1) ->
+  gen_metadata_fdef nts (getFdefLocs f1) nil f1 = Some (ex_ids,rm2) ->
+  reg_simulation mi (los,nts) gl f1 rm1 rm2 lc1 lc2 ->
   incomingValues_simulation mi re1 rm2 re2 ->
   updateValuesForNewBlock re1 lc1 rm1 = (lc1', rm1') ->
   LLVMopsem.updateValuesForNewBlock re2 lc2 = lc2' ->
-  reg_simulation mi TD gl F rm1' rm2 lc1' lc2'.
+  reg_simulation mi (los,nts) gl f1 rm1' rm2 lc1' lc2'.
 Proof.
-  induction re1; simpl; intros rm1 lc1 lc2 re2 lc1' rm1' lc2' M1 M2 mgb Hwfmi
-    Hwfg Hrsim Hisim Hupdate Hupdate'.
+  induction re1; simpl; intros rm1 lc1 lc2 re2 lc1' rm1' lc2' M1 M2 mgb ex_ids
+    nts Hwfmi Hwfg Hindom Hgetmd Hrsim Hisim Hupdate Hupdate'.
     inv Hupdate. 
     destruct re2; inv Hisim; eauto.
 
     destruct a as [[i1 gv1] [[bgv1 bgv2]|]].
       destruct re2; try solve [inv Hisim].
-      destruct p as [i2 gv2].
+      destruct p as [eid2 egv2'].
       destruct re2; try solve [inv Hisim].
       destruct p as [bid2 bgv2'].
       destruct re2; try solve [inv Hisim].
-      destruct p as [eid2 egv2'].
+      destruct p as [i2 gv2].
       destruct Hisim as [Heq [Hginj [Hlk [Hbinj [Heinj Hisim]]]]]; subst.
       remember (updateValuesForNewBlock re1 lc1 rm1) as R.      
       destruct R as [lc' rm']. inv Hupdate.
       simpl.
-      eapply reg_simulation__updateAddAL_prop'; eauto.
+      destruct Hindom as [Hin Hindom].
+      eapply reg_simulation__updateAddAL_prop; eauto.
 
       destruct re2; try solve [inv Hisim].
       destruct p as [i2 gv2].
@@ -3973,34 +2506,153 @@ Proof.
       remember (updateValuesForNewBlock re1 lc1 rm1) as R.      
       destruct R as [lc' rm']. inv Hupdate.
       simpl.
+      destruct Hindom as [Hin Hindom].
       eapply reg_simulation__updateAddAL_lc; eauto.
-        admit. admit. (*fresh*)
 Qed.
 
-Lemma switchToNewBasicBlock__reg_simulation : forall mi TD gl F rm1 rm2 lc1 lc2 
-  B1 B2 l0 ps1 cs1 tmn ps2 cs2 lc1' rm1' M1 M2 mgb
+Lemma in_getPhiNodeID__in_getPhiNodesIDs : forall p ps,
+  In p ps -> In (getPhiNodeID p) (getPhiNodesIDs ps).
+Proof.
+  induction ps; simpl; intros; auto.
+    destruct H as [H | H]; subst; auto.
+Qed.
+
+Lemma getPhiNodeID_in_getFdefLocs : forall f1 l0 ps p cs tmn,
+  blockInFdefB (block_intro l0 ps cs tmn) f1 = true ->
+  In p ps ->
+  In (getPhiNodeID p) (getFdefLocs f1).
+Proof.
+  intros.
+  destruct f1. destruct f. simpl.
+  apply in_or_app. right.
+  eapply in_getBlockLocs__in_getBlocksLocs in H; eauto.
+  simpl. 
+  apply in_or_app. left.
+  apply in_getPhiNodeID__in_getPhiNodesIDs; auto.
+Qed.  
+
+Lemma getIncomingValues_in_dom_aux : forall l0 cs1 tmn f1 TD B1 gl ps2 ps1 lc1 
+    rm1 re1,
+  blockInFdefB (block_intro l0 (ps1++ps2) cs1 tmn) f1 = true ->
+  getIncomingValuesForBlockFromPHINodes TD ps2 B1 gl lc1 rm1 = ret re1 ->
+  incomingValues_in_dom re1 (getFdefLocs f1).
+Proof.
+  induction ps2; simpl; intros ps1 lc1 rm1 re1 HBinF Hget. 
+    inv Hget. simpl. auto.
+
+    destruct a.
+    destruct (getValueViaBlockFromValuels l1 B1); tinv Hget.
+    destruct (getOperandValue TD v lc1 gl); tinv Hget.
+    remember (getIncomingValuesForBlockFromPHINodes TD ps2 B1 gl lc1 rm1) as R.
+    destruct R; tinv Hget.
+    destruct (isPointerTypB t).
+      destruct (SBopsem.get_reg_metadata TD gl rm1 v); inv Hget.
+      simpl. symmetry in HeqR.
+      rewrite_env ((ps1 ++ [insn_phi i0 t l1]) ++ ps2) in HBinF.
+      apply IHps2 with (ps1:=ps1 ++ [insn_phi i0 t l1]) in HeqR; simpl; auto.
+      split; auto.
+        eapply getPhiNodeID_in_getFdefLocs with (p:=insn_phi i0 t l1); eauto.
+          simpl. apply in_or_app. left. apply in_or_app. simpl. auto.
+      
+      inv Hget. simpl.
+      simpl. symmetry in HeqR.
+      rewrite_env ((ps1 ++ [insn_phi i0 t l1]) ++ ps2) in HBinF.
+      apply IHps2 with (ps1:=ps1 ++ [insn_phi i0 t l1]) in HeqR; simpl; auto.
+      split; auto.
+        eapply getPhiNodeID_in_getFdefLocs with (p:=insn_phi i0 t l1); eauto.
+          simpl. apply in_or_app. left. apply in_or_app. simpl. auto.
+Qed.
+
+Lemma getIncomingValues_in_dom : forall l0 cs1 tmn f1 TD B1 gl ps1 lc1 rm1 re1,
+  blockInFdefB (block_intro l0 ps1 cs1 tmn) f1 = true ->
+  getIncomingValuesForBlockFromPHINodes TD ps1 B1 gl lc1 rm1 = ret re1 ->
+  incomingValues_in_dom re1 (getFdefLocs f1).
+Proof.
+  intros.
+  eapply getIncomingValues_in_dom_aux with (ps1:=nil); eauto.
+Qed.
+
+Lemma switchToNewBasicBlock__reg_simulation : forall mi nts los gl f1 rm1 rm2 lc1
+  lc2 B1 B2 l0 ps1 cs1 tmn ps2 cs2 lc1' rm1' M1 M2 mgb ex_ids
   (Hwfmi : wf_sb_mi mgb mi M1 M2)
   (Hwfg : wf_globals mgb gl),  
-  reg_simulation mi TD gl F rm1 rm2 lc1 lc2 ->
-  switchToNewBasicBlock TD (block_intro l0 ps1 cs1 tmn) B1 gl lc1 rm1 = 
+  blockInFdefB (block_intro l0 ps1 cs1 tmn) f1 = true ->
+  gen_metadata_fdef nts (getFdefLocs f1) nil f1 = Some (ex_ids,rm2) ->
+  reg_simulation mi (los,nts) gl f1 rm1 rm2 lc1 lc2 ->
+  switchToNewBasicBlock (los,nts) (block_intro l0 ps1 cs1 tmn) B1 gl lc1 rm1 = 
     ret (lc1', rm1') ->
   label_of_block B1 = label_of_block B2 ->
   trans_phinodes rm2 ps1 = Some ps2 ->
-  exists lc2', LLVMopsem.switchToNewBasicBlock TD
+  exists lc2', LLVMopsem.switchToNewBasicBlock (los,nts)
     (block_intro l0 ps2 cs2 tmn) B2 gl lc2 = Some lc2' /\
-    reg_simulation mi TD gl F rm1' rm2 lc1' lc2'.
+    reg_simulation mi (los,nts) gl f1 rm1' rm2 lc1' lc2'.
 Proof.
-  intros mi TD gl F rm1 rm2 lc1 lc2 B1 B2 l0 ps1 cs1 tmn ps2 cs2 lc1' rm1' M1 M2
-    mgb Hwfmi Hwfg Hrsim Hswitch Hleq Htphis.
+  intros mi nts los gl f1 rm1 rm2 lc1 lc2 B1 B2 l0 ps1 cs1 tmn ps2 cs2 lc1' rm1' 
+    M1 M2 mgb ex_ids Hwfmi Hwfg HBinF Hgenmd Hrsim Hswitch Hleq Htphis.
   unfold switchToNewBasicBlock in Hswitch.
   unfold LLVMopsem.switchToNewBasicBlock. simpl in *.
-  remember (getIncomingValuesForBlockFromPHINodes TD ps1 B1 gl lc1 rm1) as R.
+  remember (getIncomingValuesForBlockFromPHINodes (los,nts) ps1 B1 gl lc1 rm1) 
+    as R.
   destruct R; try solve [inv Hswitch].  
     symmetry in HeqR.
+    assert (Hindom := HeqR).
+    eapply getIncomingValues_in_dom in Hindom; eauto.
     eapply getIncomingValuesForBlockFromPHINodes__reg_simulation in HeqR; eauto.
     destruct HeqR as [re2 [Hget Hisim]].
     rewrite Hget. inv Hswitch.
     eapply updateValuesForNewBlock__reg_simulation in H0; eauto.
+Qed.
+
+Lemma getCmdID_in_getFdefLocs : forall B f1 c cs tmn2 id0
+  (HBinF : blockInFdefB B f1 = true)
+  (Heqb1 : exists l1, exists ps1, exists cs11, 
+                B = block_intro l1 ps1 (cs11 ++ c :: cs) tmn2)
+  (Hget : getCmdID c = Some id0),
+  In id0 (getFdefLocs f1).
+Proof.
+  intros.
+  destruct Heqb1 as [l1 [ps1 [cs11 Heqb1]]]; subst.
+  destruct f1. destruct f. simpl.
+  destruct (split a).
+  apply in_or_app. right.
+  eapply in_getBlockLocs__in_getBlocksLocs in HBinF; eauto.
+  simpl. 
+  apply in_or_app. right.
+  apply in_or_app. left.
+  apply getCmdID_in_getCmdsLocs with (c:=c); auto.
+  apply in_or_app. simpl. auto.
+Qed.  
+
+Lemma ids2atoms_app : forall d1 d2,
+  ids2atoms (d1++d2) [=] ids2atoms d1 `union` ids2atoms d2.
+Proof.
+  induction d1; intros; simpl.
+    fsetdec.
+    rewrite IHd1. fsetdec.
+Qed.
+
+Lemma wf_value_id__in_getFdefLocs : forall S m f v t,
+  wf_value S m f v t -> sb_ds_sim.getValueID v[<=]ids2atoms (getFdefLocs f).
+Proof.
+  intros.
+  inv H; simpl.
+    clear. fsetdec.
+
+    destruct f. destruct f. simpl in *.
+    remember (lookupTypViaIDFromArgs a id5) as R.
+    apply ids2atoms__in.
+    destruct R; inv H2.
+      symmetry in HeqR.
+      destruct (In_dec eq_atom_dec id5 (getArgsIDs a)) as [Hin | Hnotin].
+        apply in_or_app. auto.
+
+        apply NotInArgsIDs_lookupTypViaIDFromArgs in Hnotin.
+        rewrite HeqR in Hnotin. inv Hnotin.
+      destruct (In_dec eq_atom_dec id5 (getBlocksLocs b)) as [Hin | Hnotin].
+        apply in_or_app. auto.
+        
+        apply notInBlocks__lookupTypViaIDFromBlocks in Hnotin.
+        rewrite H3 in Hnotin. inv Hnotin.
 Qed.
 
 (*****************************)
